adapt proof of termination

Weidenbach_Book/Watched_Literals/Watched_Literals_Algorithm_Restart.thy
@@ -1,6 +1,5 @@
 theory Watched_Literals_Algorithm_Restart
 imports Watched_Literals_Algorithm Watched_Literals_Transition_System_Restart
-  "../../lib/Explorer"
 begin
 
 context twl_restart_ops
@@ -15,7 +14,7 @@ definition (in -) restart_prog_pre :: \<open>'v twl_st \<Rightarrow> bool \<Righ
     (\<not>brk \<longrightarrow> get_conflict S = None)\<close>
 
 definition restart_prog
-  :: \<open>'v twl_st \<Rightarrow> nat \<Rightarrow> nat \<Rightarrow> bool \<Rightarrow> ('v twl_st \<times> nat \<times> nat) nres\<close>
+  :: \<open>'v twl_st \<Rightarrow> nat \<Rightarrow> nat \<Rightarrow> bool \<Rightarrow> (bool \<times> 'v twl_st \<times> nat \<times> nat) nres\<close>
 where
   \<open>restart_prog S m n brk = do {
      ASSERT(restart_prog_pre S brk);
@@ -23,17 +22,17 @@ where
      b2 \<leftarrow> SPEC(\<lambda>_. b \<longrightarrow> size (get_all_learned_clss S) > m);
      if b2 \<and> b \<and> \<not>brk then do {
        T \<leftarrow> SPEC(\<lambda>T. cdcl_twl_restart_only S T);
-       RETURN (T, size (get_all_learned_clss T), n)
+       RETURN (True, T, size (get_all_learned_clss T), n)
      }
      else
      if b \<and> \<not>brk then do {
        T \<leftarrow> SPEC(\<lambda>T. cdcl_twl_restart S T);
        U \<leftarrow> SPEC(\<lambda>U. cdcl_twl_stgy\<^sup>*\<^sup>* T U \<and> clauses_to_update U = {#} \<and>
           get_conflict U = None);
-       RETURN (U, size (get_all_learned_clss U), n + 1)
+       RETURN (True, U, size (get_all_learned_clss U), n + 1)
      }
      else
-       RETURN (S, m, n)
+       RETURN (False, S, m, n)
    }\<close>
 
 fun cdcl_twl_stgy_restart_prog_inv where
@@ -47,31 +46,87 @@ fun cdcl_twl_stgy_restart_prog_inv where
 lemmas cdcl_twl_stgy_restart_prog_inv_def[simp del] =
   cdcl_twl_stgy_restart_prog_inv.simps
 
+text \<open>
+  In the main loop, and purely to simplify the proof, we remember the state obtained after the last
+  restart in order to relate it to the number of clauses. In a first proof attempt, we try to make
+  do without it by only assuming its existence, but we could no prove that the loop terminates,
+  because the state can change each time.
+
+  This state is not needed at all in the execution and will be removed in the next refinement step.
+\<close>
 definition cdcl_twl_stgy_restart_prog :: "'v twl_st \<Rightarrow> 'v twl_st nres" where
   \<open>cdcl_twl_stgy_restart_prog S\<^sub>0 =
   do {
-    (brk, T, _, _, _) \<leftarrow> WHILE\<^sub>T\<^bsup>cdcl_twl_stgy_restart_prog_inv S\<^sub>0\<^esup>
+    (brk, _, T, _, _) \<leftarrow> WHILE\<^sub>T\<^bsup>cdcl_twl_stgy_restart_prog_inv S\<^sub>0\<^esup>
       (\<lambda>(brk, _). \<not>brk)
       (\<lambda>(brk, S, S', m, n).
       do {
-        T \<leftarrow> unit_propagation_outer_loop S;
+        T \<leftarrow> unit_propagation_outer_loop S';
         (brk, T) \<leftarrow> cdcl_twl_o_prog T;
-        (T, m', n') \<leftarrow> restart_prog T m n brk;
-        RETURN (brk, T, T, m', n')
+        (b, T, m', n') \<leftarrow> restart_prog T m n brk;
+        RETURN (brk, if b then T else S, T, m', n')
       })
       (False, S\<^sub>0, S\<^sub>0, size (get_all_learned_clss S\<^sub>0), 0);
     RETURN T
   }\<close>
+
+abbreviation cdcl_algo_termination_rel :: \<open>((bool \<times> 'v twl_st \<times> 'v twl_st \<times> nat \<times> nat) \<times> _) set\<close> where
+  \<open>cdcl_algo_termination_rel \<equiv>
+    {((brkT, T, T', n, n'), brkS, S, _, m, m').
+                              twl_struct_invs S \<and>
+                              \<not> brkS \<and>
+                              cdcl_twl_stgy_restart_with_leftovers1
+                             (S, m', \<not>brkS) (T, n', \<not>brkT)} \<union>
+                           {((brkT, T, T', n, n'), (brkS, S, S', m, m')). S = T \<and> \<not> brkS \<and> n' = m' \<and>
+                             twl_struct_invs S' \<and> cdcl_twl_stgy\<^sup>+\<^sup>+ S' T'} \<union>
+                           {((brkT, T), brkS, S). S = T \<and> brkT \<and> \<not> brkS}\<close>
+
+abbreviation cdcl_algo_termination_early_rel
+  :: \<open>((bool \<times> bool \<times> 'v twl_st \<times> 'v twl_st \<times> nat \<times> nat) \<times> _) set\<close>
+where
+  \<open>cdcl_algo_termination_early_rel \<equiv>
+    {((ebrkT, brkT, T, T', n, n'), ebrkS, brkS, S, _, m, m').
+                              twl_struct_invs S \<and>
+                              \<not> brkS \<and>
+                              cdcl_twl_stgy_restart_with_leftovers1
+                             (S, m', \<not>brkS) (T, n', \<not>brkT)} \<union>
+    {((ebrkT, brkT, T, T', n, n'), (ebrkS, brkS, S, S', m, m')). S = T \<and> \<not> brkS\<and> \<not> ebrkS \<and> n' = m' \<and>
+                             twl_struct_invs S' \<and> cdcl_twl_stgy\<^sup>+\<^sup>+ S' T'} \<union>
+    {((ebrkT, brkT, T), ebrkS, brkS, S). S = T \<and> (ebrkT \<or> brkT) \<and> \<not> brkS \<and> brkT}\<close>
 end
+
 
 context twl_restart
 begin
 
+lemma  wf_cdcl_algo_termination_early_rel: \<open>wf cdcl_algo_termination_early_rel\<close>
+  apply (rule wf_union_compatible)
+  apply (rule wf_union_compatible)
+  subgoal
+    by (rule wf_if_measure_in_wf[OF wf_cdcl_twl_stgy_restart_with_leftovers1,
+        of _  \<open>\<lambda>(_, brkT, T, T', n, n'). (T, n', \<not>brkT)\<close>])
+      auto
+  subgoal
+    by (rule wf_if_measure_in_wf[OF tranclp_wf_cdcl_twl_stgy,
+        of _  \<open>\<lambda>(_, brkT, T, T', n, n'). T'\<close>])
+      auto
+  subgoal
+    by auto
+  subgoal
+    by (rule wf_no_loop) auto
+  subgoal
+    by auto
+  done
+
+lemma  wf_cdcl_algo_termination_rel: \<open>wf cdcl_algo_termination_rel\<close>
+  by (rule wf_if_measure_in_wf[OF wf_cdcl_algo_termination_early_rel,
+      of _  \<open>\<lambda>(brkT, T, T', n, n'). (False, brkT, T, T', n, n')\<close>])
+    auto
 
 lemma restart_prog_spec:
   assumes
-    inv: \<open>cdcl_twl_stgy_restart_prog_inv S (brkU, U, T, m, n)\<close> and
-    cond: \<open>case (brkU, U, T, m, n) of (brk, uu_) \<Rightarrow> \<not> brk\<close> and
+    inv: \<open>(cdcl_twl_stgy_restart_prog_inv S o snd) (ebrkU, brkU, T, U, m, n)\<close> and
+    cond: \<open>case (ebrkU, brkU, T, U, m, n) of (ebrk, brk, uu_) \<Rightarrow> \<not> brk \<and> \<not>ebrk\<close> and
     other_inv: \<open>cdcl_twl_o_prog_spec V (brkT, W)\<close> and
     struct_invs_V: \<open>twl_struct_invs V\<close> and
     cp: \<open>cdcl_twl_cp\<^sup>*\<^sup>* U V\<close> and
@@ -81,19 +136,16 @@ lemma restart_prog_spec:
   shows \<open>restart_prog W m n brkT
          \<le> SPEC
             (\<lambda>x. (case x of
-                  (Ta, m', n') \<Rightarrow>
-                    RETURN (brkT, Ta, Ta, m', n'))
+                  (b, Ta, m', n') \<Rightarrow> do {
+                    ebrk \<leftarrow> RES UNIV;
+                    RETURN (ebrk, brkT, (if b then Ta else T), Ta, m', n')})
                  \<le> SPEC
-                    (\<lambda>s'. cdcl_twl_stgy_restart_prog_inv S s' \<and>
-                          (s', brkU, U, T, m, n)
-                          \<in> {((brkT, T, T', n, n'), brkS, S, S', m, m').
-                             twl_struct_invs S \<and>
-                             \<not> brkS \<and>
-                             cdcl_twl_stgy_restart_with_leftovers1
-                              (S, m', \<not>brkS) (T, n', \<not>brkT)} \<union>
-                            {((brkT, T), brkS, S). S = T \<and> brkT \<and> \<not> brkS}))\<close>
+                    (\<lambda>s'. (cdcl_twl_stgy_restart_prog_inv S o snd) s' \<and>
+                          (s', ebrkU, brkU, T, U, m, n)
+                          \<in> cdcl_algo_termination_early_rel))\<close>
+    (is \<open>_ \<le> SPEC (\<lambda>x. _ \<le> SPEC(\<lambda>s. ?I s \<and> _ \<in> ?term))\<close>)
 proof -
-  have [simp]: \<open>\<not>brkU\<close>
+  have [simp]: \<open>\<not>brkU\<close> \<open>\<not>ebrkU\<close>
     using cond by auto
   have struct_invs': \<open>cdcl_twl_restart W T' \<Longrightarrow> cdcl_twl_stgy\<^sup>*\<^sup>* T' V' \<Longrightarrow> twl_struct_invs V'\<close> for T' V'
     using assms(3) cdcl_twl_restart_twl_struct_invs
@@ -109,13 +161,14 @@ proof -
 
   have
     struct_invs_S: \<open>twl_struct_invs S\<close> and
-    struct_invs_T: \<open>twl_struct_invs T\<close> and
-    twl_stgy_invs_T: \<open>twl_stgy_invs T\<close> and
-    \<open>brkU \<longrightarrow> final_twl_state T\<close> and
-    twl_res: \<open>cdcl_twl_stgy_restart_with_leftovers (S, 0, True) m U (T, n, True)\<close> and
-    clss_T: \<open>clauses_to_update T = {#}\<close> and
-    confl: \<open>\<not> brkU \<longrightarrow> get_conflict T = None\<close>
-    using inv unfolding cdcl_twl_stgy_restart_prog_inv_def prod.case by fast+
+    struct_invs_U: \<open>twl_struct_invs U\<close> and
+    twl_stgy_invs_U: \<open>twl_stgy_invs U\<close> and
+    \<open>brkU \<longrightarrow> final_twl_state U\<close> and
+    twl_res: \<open>cdcl_twl_stgy_restart_with_leftovers (S, 0, True) m T (U, n, True)\<close> and
+    clss_T: \<open>clauses_to_update U = {#}\<close> and
+    confl: \<open>\<not> brkU \<longrightarrow> get_conflict U = None\<close>
+    using inv unfolding cdcl_twl_stgy_restart_prog_inv_def prod.case comp_def snd_conv by fast+
+
   have
     cdcl_o: \<open>cdcl_twl_o\<^sup>*\<^sup>* V W\<close> and
     conflict_W: \<open>get_conflict W \<noteq> None \<Longrightarrow> count_decided (get_trail W) = 0\<close> and
@@ -131,31 +184,27 @@ proof -
     by (meson cdcl_o assms(5) rtranclp_cdcl_twl_cp_stgyD rtranclp_cdcl_twl_o_stgyD
         rtranclp_trans)
   from twl_res have
-    STa: \<open>cdcl_twl_stgy_restart\<^sup>*\<^sup>* (S, 0, True) (U, n, True)\<close> and
-    TaT: \<open>cdcl_twl_stgy\<^sup>*\<^sup>* U T\<close> and
-    m: \<open>m = size (get_all_learned_clss U)\<close>
+    STa: \<open>cdcl_twl_stgy_restart\<^sup>*\<^sup>* (S, 0, True) (T, n, True)\<close> and
+    TaT: \<open>cdcl_twl_stgy\<^sup>*\<^sup>* T U\<close> and
+    m: \<open>m = size (get_all_learned_clss T)\<close>
     unfolding cdcl_twl_stgy_restart_with_leftovers_def prod.case snd_conv fst_conv
     by blast+
-
+  have struct_invs_T: \<open>twl_struct_invs T\<close>
+    using STa rtranclp_cdcl_twl_stgy_restart_twl_struct_invs struct_invs_S by fastforce
   have restart_prog_pre_W: \<open>restart_prog_pre W brkT\<close>
     using confl_W stgy_invs_W struct_invs_W
     unfolding restart_prog_pre_def
     by fast
-  have struct_invs_U: \<open>twl_struct_invs U\<close>
-    using rtranclp_cdcl_twl_stgy_restart_twl_struct_invs[OF STa] struct_invs_S
-    by simp
 
   have UW: \<open>cdcl_twl_stgy\<^sup>*\<^sup>* U W\<close>
     by (meson \<open>cdcl_twl_stgy\<^sup>*\<^sup>* V W\<close> local.cp rtranclp_cdcl_twl_cp_stgyD rtranclp_trans)
-  have only_restart: \<open>cdcl_twl_stgy_restart_prog_inv S
-       (False, Y, Y, size (get_all_learned_clss Y), n)\<close> (is ?A) and
-     only_restart_term: \<open>((False, Y, Y, size (get_all_learned_clss Y), n),
-        brkU, U, T, m, n)
-        \<in> {((brkT, T, T', n, n'), brkS, S, S', m, m').
-        twl_struct_invs S \<and>
-        \<not> brkS \<and>
-        cdcl_twl_stgy_restart_with_leftovers1 (S, m', \<not>brkS) (T, n', \<not>brkT)} \<union>
-        {((brkT, T), brkS, S). S = T \<and> brkT \<and> \<not> brkS}\<close> (is ?B)
+    have TW: \<open>cdcl_twl_stgy\<^sup>*\<^sup>* T W\<close>
+      by (metis (no_types) TaT \<open>cdcl_twl_stgy\<^sup>*\<^sup>* V W\<close> local.cp
+        rtranclp_cdcl_twl_cp_stgyD rtranclp_tranclp_tranclp rtranclp_unfold)
+  have only_restart: \<open>?I (ebrk, False, if True then Y else T, Y, size (get_all_learned_clss Y), n)\<close> (is ?A) and
+     only_restart_term: \<open>((ebrk, False, (if True then Y else T), Y, size (get_all_learned_clss Y), n),
+        ebrkU, brkU, T, U, m, n)
+        \<in> ?term\<close> (is ?B)
     if
       \<open>True \<longrightarrow> f n < size (get_all_learned_clss W) - m\<close> and
       m_size_W: \<open>True \<longrightarrow> m < size (get_all_learned_clss W)\<close> and
@@ -163,8 +212,17 @@ proof -
       brkX and
       X and
       \<open>\<not> brkT\<close>
-    for X brkX Y
+    for X brkX Y ebrk
   proof -
+    have \<open>size (get_all_learned_clss T) \<le> size (get_all_learned_clss U)\<close>
+      using rtranclp_cdcl_twl_stgy_size_get_all_learned[of T U] TaT
+      by auto
+    have TW: \<open>cdcl_twl_stgy\<^sup>+\<^sup>+ T W\<close>
+      by (metis (no_types) TaT \<open>cdcl_twl_stgy\<^sup>*\<^sup>* V W\<close> lits_to_upd_W lits_to_update local.cp
+        rtranclp_cdcl_twl_cp_stgyD rtranclp_tranclp_tranclp rtranclp_unfold that(6))
+    have UW: \<open>cdcl_twl_stgy\<^sup>+\<^sup>+ U W\<close>
+      by (metis (mono_tags) Nitpick.rtranclp_unfold \<open>cdcl_twl_stgy\<^sup>*\<^sup>* V W\<close> lits_to_upd_W
+        lits_to_update local.cp that(6) tranclp_cdcl_twl_cp_stgyD tranclp_rtranclp_tranclp)
     have \<open>twl_struct_invs Y\<close>
       using WY cdcl_twl_restart_only_twl_struct_invs struct_invs_W by blast
     moreover have \<open>twl_stgy_invs Y\<close>
@@ -172,13 +230,9 @@ proof -
     moreover have \<open>clauses_to_update Y = {#}\<close> \<open>get_conflict Y = None\<close>
       using WY by (auto simp: cdcl_twl_restart_only.simps)
     moreover {
-      have \<open>cdcl_twl_stgy_restart (U, n, True) (Y, n, True)\<close>
-        apply (rule restart_noGC[OF _ _ WY])
-        unfolding m[symmetric]
-        defer
-        apply (auto simp: m_size_W UW)[]
-        by (metis (mono_tags, hide_lams) Nitpick.rtranclp_unfold \<open>cdcl_twl_stgy\<^sup>*\<^sup>* V W\<close> UW lits_to_upd_W
-          lits_to_update local.cp that(6) tranclp_cdcl_twl_cp_stgyD tranclp_rtranclp_tranclp)
+      have \<open>cdcl_twl_stgy_restart (T, n, True) (Y, n, True)\<close>
+        by (rule restart_noGC[OF _ _ WY])
+         (auto simp: m_size_W UW TW  m[symmetric])
       then have \<open>cdcl_twl_stgy_restart_with_leftovers (S, 0, True)
         (size (get_all_learned_clss Y)) Y (Y, n, True)\<close>
         using STa
@@ -187,24 +241,17 @@ proof -
     }
     ultimately show ?A
       using struct_invs_S
-      unfolding cdcl_twl_stgy_restart_prog_inv_def
-      by auto
-    have \<open>cdcl_twl_stgy_restart_with_leftovers1 (U, n, True) (Y, n, True)\<close>
+      by (auto simp: cdcl_twl_stgy_restart_prog_inv_def)
+    have \<open>cdcl_twl_stgy_restart_with_leftovers1 (T, n, True) (Y, n, True)\<close>
       using m_size_W
       unfolding cdcl_twl_stgy_restart_with_leftovers1_def m
-      apply (auto intro!: cdcl_twl_stgy_restart.intros(2)[of _ W] simp: WY)[]
-      by (metis Nitpick.rtranclp_unfold UW nat_neq_iff)
-    then show ?B by (auto simp: struct_invs_U m)
+      by (auto intro!: cdcl_twl_stgy_restart.intros(2)[of _ W] simp: WY TW UW)
+    then show ?B by (auto simp: struct_invs_T m)
   qed
-  have full_restart: \<open>cdcl_twl_stgy_restart_prog_inv S (False, Z, Z, size (get_all_learned_clss Z), n + 1)\<close> (is ?A)and
+  have full_restart: \<open>?I (ebrk, False, if True then Z else T, Z, size (get_all_learned_clss Z), n + 1)\<close> (is ?A)and
     full_restart_term:
-      \<open>((False, Z, Z, size (get_all_learned_clss Z), n + 1), brkU, U, T, m, n)
-    \<in> {((brkT, T, T', n, n'), brkS, S, S', m, m').
-       twl_struct_invs S \<and>
-       \<not> brkS \<and>
-       cdcl_twl_stgy_restart_with_leftovers1 (S, m', \<not> brkS)
-        (T, n', \<not> brkT)} \<union>
-      {((brkT, T), brkS, S). S = T \<and> brkT \<and> \<not> brkS}\<close> (is ?B)
+      \<open>((ebrk, False, if True then Z else T, Z, size (get_all_learned_clss Z), n + 1), ebrkU, brkU, T, U, m, n)
+    \<in> ?term\<close> (is ?B)
     if
       \<open>restart_prog_pre W False\<close> and
       m_size: \<open>True \<longrightarrow> f n < size (get_all_learned_clss W) - m\<close> and
@@ -216,13 +263,16 @@ proof -
       YZ: \<open>cdcl_twl_stgy\<^sup>*\<^sup>* Y Z\<close> and
       clss_Z: \<open>clauses_to_update Z = {#}\<close> and
       confl_Z: \<open>get_conflict Z = None\<close>
-    for X brkX Y Z
+    for X brkX Y Z ebrk
   proof -
+    have TW: \<open>cdcl_twl_stgy\<^sup>+\<^sup>+ T W\<close>
+      by (metis (no_types) TaT \<open>cdcl_twl_stgy\<^sup>*\<^sup>* V W\<close> lits_to_upd_W lits_to_update local.cp
+        rtranclp_cdcl_twl_cp_stgyD rtranclp_tranclp_tranclp rtranclp_unfold that(7))
     have UW: \<open>cdcl_twl_stgy\<^sup>+\<^sup>+ U W\<close>
       by (metis (mono_tags) Nitpick.rtranclp_unfold \<open>cdcl_twl_stgy\<^sup>*\<^sup>* V W\<close> lits_to_upd_W
         lits_to_update local.cp that(7) tranclp_cdcl_twl_cp_stgyD tranclp_rtranclp_tranclp)
-    have UZ: \<open>cdcl_twl_stgy_restart (U, n, True) (Z, Suc n, True)\<close>
-      apply (rule restart_step[OF UW _ WY YZ])
+    have UZ: \<open>cdcl_twl_stgy_restart (T, n, True) (Z, Suc n, True)\<close>
+      apply (rule restart_step[OF TW _ WY YZ])
       using m_size
       unfolding m[symmetric]
       by (auto simp: m UW clss_Z confl_Z)
@@ -236,13 +286,44 @@ proof -
         by (auto simp: cdcl_twl_stgy_restart_with_leftovers_def)
     ultimately show ?A
       using struct_invs_S YZ WY clss_Z confl_Z
-      unfolding cdcl_twl_stgy_restart_prog_inv_def
-      by auto
-    have \<open>cdcl_twl_stgy_restart_with_leftovers1 (U, n, True) (Z, Suc n, True)\<close>
+      by (auto simp: cdcl_twl_stgy_restart_prog_inv_def)
+    have \<open>cdcl_twl_stgy_restart_with_leftovers1 (T, n, True) (Z, Suc n, True)\<close>
       using UZ by (auto simp: cdcl_twl_stgy_restart_with_leftovers1_def)
     then show ?B
-      by (auto simp: struct_invs_U)
+      by (auto simp: struct_invs_T)
   qed
+  have no_restart: \<open>?I (ebrk, brkT, if False then W else T, W, m, n)\<close>
+    for ebrk :: bool
+    using struct_invs_S STa TW
+    by (auto simp: struct_invs_S struct_invs_W stgy_invs_W clss_to_upd_W confl_W
+      cdcl_twl_stgy_restart_with_leftovers_def m brk'_no_step cdcl_twl_stgy_restart_prog_inv_def)
+
+  have no_restart_term: \<open>cdcl_twl_stgy_restart_with_leftovers1 (U, n, True) (W, n, \<not> brkT)\<close>
+  proof -
+    have \<open>cdcl_twl_stgy\<^sup>+\<^sup>+ U W\<close> if \<open>\<not> cdcl_twl_stgy_restart (U, n, True) (W, n, \<not> brkT)\<close>
+    proof -
+      have "(\<not> brkT \<or> \<not> cdcl_twl_stgy\<^sup>*\<^sup>* U W) \<or> \<not> pcdcl_twl_final_state W"
+        using twl_restart_ops.cdcl_twl_stgy_restart.restart_full that by fastforce
+      then show "cdcl_twl_stgy\<^sup>+\<^sup>+ U W"
+        by (metis (no_types) Nitpick.rtranclp_unfold \<open>cdcl_twl_stgy\<^sup>*\<^sup>* V W\<close> brk'_no_step
+          final_twl_state_def lits_to_upd_W lits_to_update local.cp pcdcl_twl_final_state_def
+          rtranclp_cdcl_twl_cp_stgyD tranclp_rtranclp_tranclp)
+    qed
+    moreover have False if \<open>\<not>cdcl_twl_stgy_restart (U, n, True) (W, n, False)\<close> and brkT
+      using UW brk'_no_step final_twl_state_def pcdcl_twl_final_state_def that
+        twl_restart_ops.cdcl_twl_stgy_restart.restart_full by blast
+    ultimately show ?thesis
+      by (auto simp: cdcl_twl_stgy_restart_with_leftovers1_def)
+  qed
+  have \<open>cdcl_twl_stgy\<^sup>+\<^sup>+ U W \<or> U = W\<close>
+    by (meson UW rtranclp_unfold)
+  then have no_restart_term: \<open>((ebrk, brkT, if False then W else T, W, m, n), ebrkU, brkU, T, U, m, n)
+    \<in> ?term\<close> for ebrk
+    using no_restart_term
+    apply (auto simp: struct_invs_T struct_invs_U)
+    by (metis (no_types, lifting) \<open>cdcl_twl_stgy\<^sup>*\<^sup>* V W\<close> lits_to_upd_W lits_to_update local.cp
+      rtranclp_cdcl_twl_cp_stgyD rtranclp_into_tranclp1 rtranclp_unfold tranclp_idemp)+
+
   show ?thesis
     unfolding restart_prog_def restart_required_def
     apply (refine_vcg; remove_dummy_vars)
@@ -255,367 +336,53 @@ proof -
       by (rule full_restart)
     subgoal for X brkX Y Z
       by (rule full_restart_term)
-    subgoal for X brkX
-        
-qed
-
-lemma (in twl_restart)
-  assumes
-    inv: \<open>case (brk, T, m, n) of  (brk, T, m, n) \<Rightarrow> cdcl_twl_stgy_restart_prog_inv S brk T m n\<close> and
-    cond: \<open>case (brk, T, m, n) of (brk, uu_) \<Rightarrow> \<not> brk\<close> and
-    other_inv: \<open>cdcl_twl_o_prog_spec S' (brk', U)\<close> and
-    struct_invs_S: \<open>twl_struct_invs S'\<close> and
-    cp: \<open>cdcl_twl_cp\<^sup>*\<^sup>* T S'\<close> and
-    lits_to_update: \<open>literals_to_update S' = {#}\<close> and
-    \<open>\<forall>S'a. \<not> cdcl_twl_cp S' S'a\<close> and
-    \<open>twl_stgy_invs S'\<close> and
-    brk: \<open>(brk', brk) \<in> bool_rel\<close>
-  shows restart_prog_spec:
-    \<open>restart_prog U m n brk'
-         \<le> SPEC
-             (\<lambda>x. (case x of
-                   (T, m, na) \<Rightarrow> RETURN (brk', T, m, na))
-                  \<le> SPEC
-                      (\<lambda>s'. (case s' of
-  (brk, T, m, n'') \<Rightarrow>
-    twl_struct_invs T \<and>
-    twl_stgy_invs T \<and>
-    (brk \<longrightarrow> final_twl_state T) \<and>
-    cdcl_twl_stgy_restart_with_leftovers (S, 0, \<not>brk) m S (T, n'', \<not>brk) \<and>
-    clauses_to_update T = {#} \<and>
-    (\<not> brk \<longrightarrow> get_conflict T = None)) \<and>
- (s', brk, T, n)
- \<in> {((brkT, T, m, n'), brkS, S, _).
-     twl_struct_invs S \<and>
-     cdcl_twl_stgy_restart_with_leftovers1 (S, n, \<not>brkS) (T, n', \<not>brkS)} \<union>
-    {((brkT, T, _, _), brkS, S, _). S = T \<and> brkT \<and> \<not> brkS}))\<close> (is ?A)
-proof -
-  have brk[simp]: \<open>brk' = brk\<close>
-    using brk by auto
-  have struct_invs': \<open>cdcl_twl_restart U T \<Longrightarrow> cdcl_twl_stgy\<^sup>*\<^sup>* T V \<Longrightarrow> twl_struct_invs V\<close> for T V
-    using assms(3) cdcl_twl_restart_twl_struct_invs
-    by (metis (no_types, lifting) case_prodD rtranclp_cdcl_twl_stgy_twl_struct_invs)
-  have stgy_invs: \<open>cdcl_twl_restart U V \<Longrightarrow> cdcl_twl_stgy\<^sup>*\<^sup>* V W \<Longrightarrow> twl_stgy_invs W\<close> for V W
-    using assms(3) cdcl_twl_restart_twl_stgy_invs
-    by (metis (no_types, lifting) case_prodD cdcl_twl_restart_twl_struct_invs
-      rtranclp_cdcl_twl_stgy_twl_stgy_invs)
-  have res_no_clss_to_upd: \<open>cdcl_twl_restart U V \<Longrightarrow> clauses_to_update V = {#}\<close> for V
-    by (auto simp: cdcl_twl_restart.simps)
-  have res_no_confl: \<open>cdcl_twl_restart U V \<Longrightarrow> get_conflict V = None\<close> for V
-    by (auto simp: cdcl_twl_restart.simps)
-
-  have
-    struct_invs_T: \<open>twl_struct_invs T\<close> and
-    \<open>twl_stgy_invs T\<close> and
-    \<open>brk \<longrightarrow> final_twl_state T\<close> and
-    twl_res: \<open>cdcl_twl_stgy_restart_with_leftovers (S, 0, True) m (T, n, True)\<close> and
-    \<open>clauses_to_update T = {#}\<close> and
-    confl: \<open>\<not> brk \<longrightarrow> get_conflict T = None\<close>
-    using inv unfolding cdcl_twl_stgy_restart_prog_inv_def prod.case by fast+
-  have
-    cdcl_o: \<open>cdcl_twl_o\<^sup>*\<^sup>* S' U\<close> and
-    conflict_U: \<open>get_conflict U \<noteq> None \<Longrightarrow> count_decided (get_trail U) = 0\<close> and
-    brk'_no_step: \<open>brk' \<Longrightarrow> final_twl_state U\<close> and
-    struct_invs_U: \<open>twl_struct_invs U\<close> and
-    stgy_invs_U: \<open>twl_stgy_invs U\<close> and
-    clss_to_upd_U: \<open>clauses_to_update U = {#}\<close> and
-    lits_to_upd_U: \<open>\<not> brk' \<longrightarrow> literals_to_update U \<noteq> {#}\<close> and
-    confl_U: \<open>\<not> brk' \<longrightarrow> get_conflict U = None\<close>
-    using other_inv unfolding final_twl_state_def by fast+
-
-  have \<open>cdcl_twl_stgy\<^sup>*\<^sup>* T U\<close>
-    by (meson \<open>cdcl_twl_o\<^sup>*\<^sup>* S' U\<close> assms(5) rtranclp_cdcl_twl_cp_stgyD rtranclp_cdcl_twl_o_stgyD
-        rtranclp_trans)
-  from twl_res obtain Ta where
-    STa: \<open>cdcl_twl_stgy_restart\<^sup>*\<^sup>* (S, 0, True) (Ta, n, True)\<close> and
-    TaT: \<open>cdcl_twl_stgy\<^sup>*\<^sup>* Ta T\<close> and
-    m: \<open>m = size (get_all_learned_clss Ta)\<close>
-    unfolding cdcl_twl_stgy_restart_with_leftovers_def prod.case snd_conv fst_conv
-    by blast
-  have
-    twl_restart_after_restart:
-      \<open>cdcl_twl_stgy_restart (Ta, n, \<not>False) (W, Suc n, \<not>False)\<close> and
-    rtranclp_twl_restart_after_restart:
-      \<open>cdcl_twl_stgy_restart\<^sup>*\<^sup>* (S, 0, \<not>False) (W, n + 1, \<not>False)\<close> and
-    cdcl_twl_stgy_restart_with_leftovers_after_restart:
-      \<open>cdcl_twl_stgy_restart_with_leftovers (S, 0, \<not>False) (size (get_all_learned_clss W))
-        (W, n + 1, \<not>False)\<close> and
-    cdcl_twl_stgy_restart_with_leftovers_after_restart_T_V:
-    \<open>cdcl_twl_stgy_restart_with_leftovers (Ta, n, \<not>False) (size (get_all_learned_clss W))
-         (W, Suc n, \<not>False)\<close> and
-    cdcl_twl_stgy_restart_with_leftovers1_after_restart:
-      \<open>cdcl_twl_stgy_restart_with_leftovers1 (Ta, n, \<not>False) (W, Suc n, \<not>False)\<close>
-    if
-      f: \<open>True \<longrightarrow> f (snd (U, n)) < size (get_all_learned_clss (fst (U, n))) - m\<close> and
-      res: \<open>cdcl_twl_restart U V\<close> and
-      pre: \<open>cdcl_twl_stgy\<^sup>*\<^sup>* V W\<close> and
-      [unfolded brk, simp]: \<open>brk' = False\<close>
-    for V W
-  proof -
-    have \<open>S' \<noteq> U\<close>
-      using lits_to_update lits_to_upd_U by auto
-    then have \<open>cdcl_twl_o\<^sup>+\<^sup>+ S' U\<close>
-      using \<open>cdcl_twl_o\<^sup>*\<^sup>* S' U\<close> unfolding rtranclp_unfold by auto
-    then have st: \<open>cdcl_twl_stgy\<^sup>+\<^sup>+ Ta U\<close>
-      using TaT
-      by (meson local.cp rtranclp_cdcl_twl_cp_stgyD rtranclp_tranclp_tranclp
-          tranclp_cdcl_twl_o_stgyD)
-
-    show twl_res_T_V[unfolded not_False_eq_True]:
-      \<open>cdcl_twl_stgy_restart (Ta, n, \<not>False) (W, Suc n, \<not>False)\<close>
-      unfolding not_False_eq_True
-      apply (rule cdcl_twl_stgy_restart.restart_step[of _ U _ V])
-      subgoal by (rule st)
-      subgoal using f unfolding m by simp
-      subgoal by (rule res)
-      subgoal using pre by simp
-      done
-    show \<open>cdcl_twl_stgy_restart_with_leftovers (Ta, n, \<not>False)
-        (size (get_all_learned_clss W)) (W, Suc n, \<not>False)\<close>
-      unfolding not_False_eq_True cdcl_twl_stgy_restart_with_leftovers_def
-      by (rule exI[of _ \<open>W\<close>])(auto simp: twl_res_T_V)
-    show \<open>cdcl_twl_stgy_restart\<^sup>*\<^sup>* (S, 0, \<not>False) (W, n + 1, \<not>False)\<close>
-      using twl_res twl_res_T_V STa
-      unfolding cdcl_twl_stgy_restart_with_leftovers_def apply -
-      by (auto dest: cdcl_twl_stgy_restart_cdcl_twl_stgy_cdcl_twl_stgy_restart)
-    then show  \<open>cdcl_twl_stgy_restart_with_leftovers (S, 0, \<not>False) (size (get_all_learned_clss W))
-        (W, n + 1, \<not>False)\<close>
-      unfolding cdcl_twl_stgy_restart_with_leftovers_def apply -
-      by (rule exI[of _ W]) auto
-    show \<open>cdcl_twl_stgy_restart_with_leftovers1 (Ta, n, \<not>False) (W, Suc n, \<not>False)\<close>
-      using twl_res_T_V
-      unfolding cdcl_twl_stgy_restart_with_leftovers1_def not_False_eq_True
-      by fast
-  qed
-  let ?m = \<open>\<lambda>W. (size (get_all_learned_clss W))\<close>
-  have
-    twl_restart_after_restart_only:
-      \<open>cdcl_twl_stgy_restart (Ta, n, \<not>False) (V, n, \<not>False)\<close> and
-    rtranclp_twl_restart_after_restart_only:
-      \<open>cdcl_twl_stgy_restart\<^sup>*\<^sup>* (S, 0, \<not>False) (V, n, \<not>False)\<close> and
-    cdcl_twl_stgy_restart_with_leftovers_after_restart_only:
-      \<open>cdcl_twl_stgy_restart_with_leftovers (S, 0, \<not>False) (?m V) (V, n, \<not>False)\<close> and
-    cdcl_twl_stgy_restart_with_leftovers_after_restart_T_V:
-      \<open>cdcl_twl_stgy_restart_with_leftovers (Ta, n, \<not>False) (?m V) (V, n, \<not>False)\<close> and
-    cdcl_twl_stgy_restart_with_leftovers1_after_restart_only:
-    \<open>cdcl_twl_stgy_restart_with_leftovers1 (Ta, n, \<not>False) (V, n, \<not>False)\<close>
-    if
-      f: \<open>True \<longrightarrow> m < size (get_all_learned_clss U)\<close> and
-      res: \<open>cdcl_twl_restart_only U V\<close> and
-      [unfolded brk, simp]: \<open>brk' = False\<close>
-    for V
-  proof -
-    have \<open>S' \<noteq> U\<close>
-      using lits_to_update lits_to_upd_U by auto
-    then have \<open>cdcl_twl_o\<^sup>+\<^sup>+ S' U\<close>
-      using \<open>cdcl_twl_o\<^sup>*\<^sup>* S' U\<close> unfolding rtranclp_unfold by auto
-    then have st: \<open>cdcl_twl_stgy\<^sup>+\<^sup>+ Ta U\<close> and st2: \<open>cdcl_twl_stgy\<^sup>+\<^sup>+ T U\<close>
-      using TaT
-      by (meson local.cp rtranclp_cdcl_twl_cp_stgyD rtranclp_tranclp_tranclp
-          tranclp_cdcl_twl_o_stgyD)+
-
-    show twl_res_T_V[unfolded not_False_eq_True]:
-      \<open>cdcl_twl_stgy_restart (Ta, n, \<not>False) (V, n, \<not>False)\<close>
-      unfolding not_False_eq_True
-      apply (rule cdcl_twl_stgy_restart.restart_noGC[of _ U])
-      subgoal by (rule st)
-      subgoal using f unfolding m by simp
-      subgoal by (rule res)
-      done
-    show \<open>cdcl_twl_stgy_restart_with_leftovers (Ta, n, \<not>False) (?m V) (V, n, \<not>False)\<close>
-      unfolding not_False_eq_True cdcl_twl_stgy_restart_with_leftovers_def
-      by (rule exI[of _ \<open>V\<close>])(auto simp: twl_res_T_V)
-    show \<open>cdcl_twl_stgy_restart\<^sup>*\<^sup>* (S, 0, \<not>False) (V, n, \<not>False)\<close>
-      using twl_res twl_res_T_V TaT STa
-      unfolding cdcl_twl_stgy_restart_with_leftovers_def apply -
-      by auto
-    then show  \<open>cdcl_twl_stgy_restart_with_leftovers (S, 0, \<not>False) (?m V) (V, n, \<not>False)\<close>
-      unfolding cdcl_twl_stgy_restart_with_leftovers_def apply -
-      by (rule exI[of _ V]) auto
-    show \<open>cdcl_twl_stgy_restart_with_leftovers1 (Ta, n, \<not>False) (V, n, \<not>False)\<close>
-      using twl_res_T_V
-      unfolding cdcl_twl_stgy_restart_with_leftovers1_def not_False_eq_True
-      by fast
-  qed
-
-  have
-    rtranclp_twl_restart_after_restart_S_U:
-      \<open>cdcl_twl_stgy_restart_with_leftovers (S, 0, True) m (U, n, True)\<close> and
-    rtranclp_twl_restart_after_restart_T_U:
-      \<open>cdcl_twl_stgy_restart_with_leftovers (Ta, n, True) m (U, n, True)\<close>
-  proof -
-    have TaU: \<open>cdcl_twl_stgy\<^sup>*\<^sup>* Ta (fst (U, n))\<close>
-      using TaT \<open>cdcl_twl_stgy\<^sup>*\<^sup>* T U\<close> by auto
-    then show \<open>cdcl_twl_stgy_restart_with_leftovers (S, 0, True) m (U, n, True)\<close>
-      using STa m unfolding cdcl_twl_stgy_restart_with_leftovers_def
-      by fastforce
-    show \<open>cdcl_twl_stgy_restart_with_leftovers (Ta, n, True) m (U, n, True)\<close>
-      using \<open>cdcl_twl_stgy\<^sup>*\<^sup>* T U\<close> TaU m unfolding cdcl_twl_stgy_restart_with_leftovers_def
-      by fastforce
-  qed
-  have
-    rtranclp_twl_restart_after_restart_brk:
-      \<open>cdcl_twl_stgy_restart_with_leftovers (S, 0, True) m (U, n, True)\<close>
-    if
-      [simp]: \<open>brk = True\<close>
-  proof -
-    have \<open>full cdcl_twl_stgy T U \<or> get_conflict U \<noteq> None\<close>
-      using brk'_no_step \<open>cdcl_twl_stgy\<^sup>*\<^sup>* T U\<close>
-      unfolding rtranclp_unfold full_def final_twl_state_def by auto
-    then have \<open>(cdcl_twl_stgy\<^sup>*\<^sup>* T U \<and> pcdcl_twl_final_state U) \<or> get_conflict U \<noteq> None\<close>
-      unfolding full_def pcdcl_twl_final_state_def
-      by auto
-    then consider
-        (step) \<open>cdcl_twl_stgy_restart (T, n, True) (U, n, False)\<close> |
-        (final) \<open>get_conflict U \<noteq> None\<close>
-      using cdcl_twl_stgy_restart.intros(3)[of T U]
-      by (auto dest!: cdcl_twl_stgy_restart.intros)
-    then show \<open>cdcl_twl_stgy_restart_with_leftovers (S, 0, True) m (U, n, True)\<close>
-    proof cases
-      case step
-      then show ?thesis
-        using twl_res \<open>cdcl_twl_stgy\<^sup>*\<^sup>* T U\<close> unfolding cdcl_twl_stgy_restart_with_leftovers_def
-        using cdcl_twl_stgy_restart_cdcl_twl_stgy_cdcl_twl_stgy_restart2[of T n True U] apply -
-        by fastforce
-    next
-      case final
-      then show ?thesis
-        using twl_res \<open>cdcl_twl_stgy\<^sup>*\<^sup>* T U\<close>  unfolding cdcl_twl_stgy_restart_with_leftovers_def
-        by fastforce
-    qed
-  qed
-  have cdcl_twl_stgy_restart_with_leftovers1_T_U:
-    \<open>cdcl_twl_stgy_restart_with_leftovers1 (T, n, True) (U, n, True) \<longleftrightarrow> T \<noteq> U\<close>
-  proof -
-    have \<open>cdcl_twl_stgy\<^sup>+\<^sup>+ T U \<or> T = U\<close>
-      using \<open>cdcl_twl_stgy\<^sup>*\<^sup>* T U\<close> unfolding rtranclp_unfold by auto
-    then show ?thesis
-      using wf_not_refl[OF wf_cdcl_twl_stgy_restart, of \<open>(U, n, True)\<close>]
-      using wf_not_refl[OF tranclp_wf_cdcl_twl_stgy, of \<open>U\<close>]
-        struct_invs_U
-      unfolding cdcl_twl_stgy_restart_with_leftovers1_def by auto
-  qed
-  have brk'_eq: \<open>\<not>cdcl_twl_stgy_restart_with_leftovers1 (T, n, True) (U, n, True) \<Longrightarrow> brk'\<close>
-    using cdcl_o lits_to_upd_U lits_to_update local.cp
-    unfolding cdcl_twl_stgy_restart_with_leftovers1_def
-    unfolding rtranclp_unfold
-    by (auto dest!: tranclp_cdcl_twl_o_stgyD tranclp_cdcl_twl_cp_stgyD
-        simp: rtranclp_unfold
-        dest: rtranclp_tranclp_tranclp tranclp_trans)
-
-  have [simp]: \<open>brk = False\<close>
-    using cond by auto
-  show ?A
-    unfolding restart_prog_def restart_required_def
-    apply (refine_vcg; remove_dummy_vars)
-    subgoal using struct_invs_U stgy_invs_U confl_U unfolding restart_prog_pre_def by fast
-    subgoal using cdcl_twl_restart_only_twl_struct_invs struct_invs_U by blast
-    subgoal using cdcl_twl_stgy_restart_only_twl_stgy_invs stgy_invs_U by blast
-    subgoal by simp
-    subgoal by (rule cdcl_twl_stgy_restart_with_leftovers_after_restart_only)
-    subgoal by (auto simp add: cdcl_twl_restart_only.simps)
-    subgoal by (auto simp add: cdcl_twl_restart_only.simps)
-    subgoal apply (auto intro!: struct_invs_S struct_invs_T
-      cdcl_twl_stgy_restart_with_leftovers1_after_restart_only[unfolded not_False_eq_True])
-thm 
-  cdcl_twl_stgy_restart_with_leftovers1_after_restart_only[unfolded not_False_eq_True]
-
-      apply (rule 
-        cdcl_twl_stgy_restart_with_leftovers1_after_restart_only[unfolded not_False_eq_True])
-      sorry
-    subgoal by (rule struct_invs')
-    subgoal by (rule stgy_invs)
-    subgoal by simp
-    subgoal
-      by (rule cdcl_twl_stgy_restart_with_leftovers_after_restart, simp)
-    subgoal
-      using rtranclp_twl_restart_after_restart_T_U
-      by (auto intro!: struct_invs_S struct_invs_T
-        cdcl_twl_stgy_restart_with_leftovers1_after_restart[unfolded not_False_eq_True])
-    subgoal by (rule struct_invs_U)
-    subgoal by (rule stgy_invs_U)
-    subgoal by (rule brk'_no_step) simp
-    subgoal
-      by (auto intro: rtranclp_twl_restart_after_restart_brk
-        rtranclp_twl_restart_after_restart_S_U)
-    subgoal by (rule clss_to_upd_U)
-    subgoal using struct_invs_U conflict_U lits_to_upd_U
-      by (cases \<open>get_conflict U\<close>)(auto simp: twl_struct_invs_def)
-    subgoal
-      using cdcl_twl_stgy_restart_with_leftovers1_T_U brk'_eq
-      by (auto simp: twl_restart_after_restart struct_invs_S struct_invs_T
-        cdcl_twl_stgy_restart_with_leftovers_after_restart_T_V struct_invs_U
-        rtranclp_twl_restart_after_restart_brk rtranclp_twl_restart_after_restart_T_U
-        cdcl_twl_stgy_restart_with_leftovers1_after_restart)
+    subgoal for brk brk'
+      by (rule no_restart)
+    subgoal for brk brk'
+      by (rule no_restart_term)
     done
 qed
 
-lemma (in twl_restart) cdcl_twl_stgy_restart_prog_spec:
-  fixes S :: \<open>'v twl_st\<close>
+definition cdcl_twl_stgy_restart_prog_bounded :: "'v twl_st \<Rightarrow> (bool \<times> 'v twl_st) nres" where
+  \<open>cdcl_twl_stgy_restart_prog_bounded S\<^sub>0 =
+  do {
+    ebrk \<leftarrow> RES UNIV;
+    (ebrk, _, _, T, _, n) \<leftarrow> WHILE\<^sub>T\<^bsup>cdcl_twl_stgy_restart_prog_inv S\<^sub>0 o snd\<^esup>
+      (\<lambda>(ebrk, brk, _). \<not>brk \<and> \<not>ebrk)
+      (\<lambda>(ebrk, brk, S', S, m, n).
+      do {
+        T \<leftarrow> unit_propagation_outer_loop S;
+        (brk, T) \<leftarrow> cdcl_twl_o_prog T;
+        (b, T, m, n) \<leftarrow> restart_prog T m n brk;
+	ebrk \<leftarrow> RES UNIV;
+        RETURN (ebrk, brk, if b then T else S', T, m, n)
+      })
+      (ebrk, False, S\<^sub>0, S\<^sub>0, size (get_all_learned_clss S\<^sub>0), 0);
+    RETURN (ebrk, T)
+  }\<close>
+
+lemma (in twl_restart) cdcl_twl_stgy_prog_bounded_spec:
   assumes \<open>twl_struct_invs S\<close> and \<open>twl_stgy_invs S\<close> and \<open>clauses_to_update S = {#}\<close> and
     \<open>get_conflict S = None\<close>
   shows
-    \<open>cdcl_twl_stgy_restart_prog S \<le> SPEC(\<lambda>T.
-       \<exists>S' m n. cdcl_twl_stgy_restart_with_leftovers (S, 0, True) m S' (T, n, True) \<and>
-        final_twl_state T)\<close>
-    (is \<open>_ \<le> SPEC(\<lambda>T. ?P T)\<close>)
+    \<open>cdcl_twl_stgy_restart_prog_bounded S \<le> SPEC(\<lambda>(brk, T). \<exists> S' m n. (cdcl_twl_stgy_restart_with_leftovers (S, 0, True) m S' (T, n, True) \<and>
+        (\<not>brk \<longrightarrow> final_twl_state T)))\<close>
+    (is \<open>_ \<le> SPEC ?P\<close>)
 proof -
-  
-  (* have final_prop: \<open>?P T\<close>
-   *   if
-   *    inv: \<open>case (brk, T, n) of  (brk, T, m, n) \<Rightarrow> cdcl_twl_stgy_restart_prog_inv S brk T m n\<close> and
-   *     \<open>\<not> (case (brk, T, n) of (brk, uu_) \<Rightarrow> \<not> brk)\<close>
-   *   for brk T n
-   * proof -
-   *   have
-   *     \<open>brk\<close> and
-   *     \<open>twl_struct_invs T\<close> and
-   *     \<open>twl_stgy_invs T\<close> and
-   *     ns: \<open>final_twl_state T\<close> and
-   *     twl_left_overs: \<open>cdcl_twl_stgy_restart_with_leftovers (S, 0) (T, n)\<close> and
-   *     \<open>clauses_to_update T = {#}\<close>
-   *     using that unfolding cdcl_twl_stgy_restart_prog_inv_def by auto
-   *   obtain S' where
-   *      st: \<open>cdcl_twl_stgy_restart\<^sup>*\<^sup>* (S, 0) (S', n)\<close> and
-   *      S'_T: \<open>cdcl_twl_stgy\<^sup>*\<^sup>* S' T\<close>
-   *     using twl_left_overs unfolding cdcl_twl_stgy_restart_with_leftovers_def by auto
-   *   then show ?thesis
-   *     using ns unfolding cdcl_twl_stgy_restart_with_leftovers_def apply -
-   *     apply (rule_tac x=n in exI)
-   *     apply (rule conjI)
-   *     subgoal by (rule_tac x=S' in exI) auto
-   *     subgoal by auto
-   *     done
-  * qed *)
-  let ?R = \<open>{((brkT :: bool, T :: 'v twl_st, T' :: 'v twl_st, n :: nat, n' :: nat),
-      brkS, S, S' :: 'v twl_st, m :: nat, m' :: nat).
-    twl_struct_invs S \<and> \<not> brkS \<and>
-    cdcl_twl_stgy_restart_with_leftovers1 (S, m, brkS) (T, n, brkT)} \<union>
-    {((brkT, T), brkS, S). S = T \<and> brkT \<and> \<not> brkS}\<close>
-
-  have wf: \<open>wf ?R\<close>
-    apply (rule wf_union_compatible)
-    subgoal
-      by (rule wf_if_measure_in_wf[OF wf_cdcl_twl_stgy_restart_with_leftovers1,
-          of _  \<open>\<lambda>(brkT, T, T', n, n'). (T, n, brkT)\<close>])
-        auto
-    subgoal
-      by (rule wf_no_loop) auto
-    subgoal
-      by auto
-    done
-   term cdcl_twl_stgy_restart
-
   show ?thesis
     supply RETURN_as_SPEC_refine[refine2 del]
-    unfolding cdcl_twl_stgy_restart_prog_def full_def
-    apply (refine_vcg WHILEIT_rule[where R = \<open>?R\<close>];
-      remove_dummy_vars)
-    subgoal by (rule wf)
-    subgoal using assms unfolding cdcl_twl_stgy_restart_prog_inv_def cdcl_twl_stgy_restart_with_leftovers_def
-      by auto
-    subgoal using assms unfolding cdcl_twl_stgy_restart_prog_inv_def cdcl_twl_stgy_restart_with_leftovers_def
-      by (auto dest: rtranclp_cdcl_twl_stgy_restart_twl_struct_invs)
+    unfolding cdcl_twl_stgy_restart_prog_bounded_def full_def
+    apply (refine_vcg
+        WHILEIT_rule[where
+           R = \<open>cdcl_algo_termination_early_rel\<close>];
+        remove_dummy_vars)
+    subgoal
+      by (rule wf_cdcl_algo_termination_early_rel)
+    subgoal using assms
+      by (auto simp: cdcl_twl_stgy_restart_prog_inv_def cdcl_twl_stgy_restart_with_leftovers_def)
+    subgoal using assms
+      by (auto dest: rtranclp_cdcl_twl_stgy_restart_twl_struct_invs
+        simp: cdcl_twl_stgy_restart_prog_inv_def cdcl_twl_stgy_restart_with_leftovers_def)
     subgoal using assms
       by (auto simp: cdcl_twl_stgy_restart_prog_inv_def cdcl_twl_stgy_restart_with_leftovers_def
         dest!: rtranclp_cdcl_twl_stgy_restart_clauses_to_update)
@@ -632,854 +399,76 @@ proof -
         no_step_cdcl_twl_cp_no_step_cdcl\<^sub>W_cp)
     subgoal by fast
     subgoal for brkU U T m n V brkT W
-      explore_lemma
-      sorry
-
-    subgoal by (rule wf_cdcl_twl_stgy_restart_measure)
-    subgoal using assms by fast
-    subgoal using assms by fast
-    subgoal using assms by fast
-    subgoal by (rule cdcl_twl_stgy_restart_with_leftovers_refl)
-    subgoal using assms by fast
-    subgoal using assms by fast
-    subgoal by fast
-    subgoal by fast
-    subgoal by fast
-    subgoal by fast
-    subgoal by (simp add: no_step_cdcl_twl_cp_no_step_cdcl\<^sub>W_cp)
-    subgoal by fast
-    subgoal by (rule final_prop[unfolded cdcl_twl_stgy_restart_prog_inv_def])
-    done
-qed
-lemma (in twl_restart)
-  assumes
-    inv: \<open>case (brk, T, m, n) of  (brk, T, m, n) \<Rightarrow> cdcl_twl_stgy_restart_prog_inv S brk T m n\<close> and
-    cond: \<open>case (brk, T, m, n) of (brk, uu_) \<Rightarrow> \<not> brk\<close> and
-    other_inv: \<open>cdcl_twl_o_prog_spec S' (brk', U)\<close> and
-    struct_invs_S: \<open>twl_struct_invs S'\<close> and
-    cp: \<open>cdcl_twl_cp\<^sup>*\<^sup>* T S'\<close> and
-    lits_to_update: \<open>literals_to_update S' = {#}\<close> and
-    \<open>\<forall>S'a. \<not> cdcl_twl_cp S' S'a\<close> and
-    \<open>twl_stgy_invs S'\<close> and
-    brk: \<open>(brk', brk) \<in> bool_rel\<close>
-  shows restart_prog_spec:
-    \<open>restart_prog U m n brk'
-         \<le> SPEC
-             (\<lambda>x. (case x of
-                   (T, m, na) \<Rightarrow> RETURN (brk', T, m, na))
-                  \<le> SPEC
-                      (\<lambda>s'. (case s' of
-  (brk, T, m, n'') \<Rightarrow>
-    twl_struct_invs T \<and>
-    twl_stgy_invs T \<and>
-    (brk \<longrightarrow> final_twl_state T) \<and>
-    cdcl_twl_stgy_restart_with_leftovers (S, 0, \<not>brk) m S (T, n'', \<not>brk) \<and>
-    clauses_to_update T = {#} \<and>
-    (\<not> brk \<longrightarrow> get_conflict T = None)) \<and>
- (s', brk, T, n)
- \<in> {((brkT, T, m, n'), brkS, S, _).
-     twl_struct_invs S \<and>
-     cdcl_twl_stgy_restart_with_leftovers1 (S, n, \<not>brkS) (T, n', \<not>brkS)} \<union>
-    {((brkT, T, _, _), brkS, S, _). S = T \<and> brkT \<and> \<not> brkS}))\<close> (is ?A)
-proof -
-  have brk[simp]: \<open>brk' = brk\<close>
-    using brk by auto
-  have struct_invs': \<open>cdcl_twl_restart U T \<Longrightarrow> cdcl_twl_stgy\<^sup>*\<^sup>* T V \<Longrightarrow> twl_struct_invs V\<close> for T V
-    using assms(3) cdcl_twl_restart_twl_struct_invs
-    by (metis (no_types, lifting) case_prodD rtranclp_cdcl_twl_stgy_twl_struct_invs)
-  have stgy_invs: \<open>cdcl_twl_restart U V \<Longrightarrow> cdcl_twl_stgy\<^sup>*\<^sup>* V W \<Longrightarrow> twl_stgy_invs W\<close> for V W
-    using assms(3) cdcl_twl_restart_twl_stgy_invs
-    by (metis (no_types, lifting) case_prodD cdcl_twl_restart_twl_struct_invs
-      rtranclp_cdcl_twl_stgy_twl_stgy_invs)
-  have res_no_clss_to_upd: \<open>cdcl_twl_restart U V \<Longrightarrow> clauses_to_update V = {#}\<close> for V
-    by (auto simp: cdcl_twl_restart.simps)
-  have res_no_confl: \<open>cdcl_twl_restart U V \<Longrightarrow> get_conflict V = None\<close> for V
-    by (auto simp: cdcl_twl_restart.simps)
-
-  have
-    struct_invs_T: \<open>twl_struct_invs T\<close> and
-    \<open>twl_stgy_invs T\<close> and
-    \<open>brk \<longrightarrow> final_twl_state T\<close> and
-    twl_res: \<open>cdcl_twl_stgy_restart_with_leftovers (S, 0, True) m (T, n, True)\<close> and
-    \<open>clauses_to_update T = {#}\<close> and
-    confl: \<open>\<not> brk \<longrightarrow> get_conflict T = None\<close>
-    using inv unfolding cdcl_twl_stgy_restart_prog_inv_def prod.case by fast+
-  have
-    cdcl_o: \<open>cdcl_twl_o\<^sup>*\<^sup>* S' U\<close> and
-    conflict_U: \<open>get_conflict U \<noteq> None \<Longrightarrow> count_decided (get_trail U) = 0\<close> and
-    brk'_no_step: \<open>brk' \<Longrightarrow> final_twl_state U\<close> and
-    struct_invs_U: \<open>twl_struct_invs U\<close> and
-    stgy_invs_U: \<open>twl_stgy_invs U\<close> and
-    clss_to_upd_U: \<open>clauses_to_update U = {#}\<close> and
-    lits_to_upd_U: \<open>\<not> brk' \<longrightarrow> literals_to_update U \<noteq> {#}\<close> and
-    confl_U: \<open>\<not> brk' \<longrightarrow> get_conflict U = None\<close>
-    using other_inv unfolding final_twl_state_def by fast+
-
-  have \<open>cdcl_twl_stgy\<^sup>*\<^sup>* T U\<close>
-    by (meson \<open>cdcl_twl_o\<^sup>*\<^sup>* S' U\<close> assms(5) rtranclp_cdcl_twl_cp_stgyD rtranclp_cdcl_twl_o_stgyD
-        rtranclp_trans)
-  from twl_res obtain Ta where
-    STa: \<open>cdcl_twl_stgy_restart\<^sup>*\<^sup>* (S, 0, True) (Ta, n, True)\<close> and
-    TaT: \<open>cdcl_twl_stgy\<^sup>*\<^sup>* Ta T\<close> and
-    m: \<open>m = size (get_all_learned_clss Ta)\<close>
-    unfolding cdcl_twl_stgy_restart_with_leftovers_def prod.case snd_conv fst_conv
-    by blast
-  have
-    twl_restart_after_restart:
-      \<open>cdcl_twl_stgy_restart (Ta, n, \<not>False) (W, Suc n, \<not>False)\<close> and
-    rtranclp_twl_restart_after_restart:
-      \<open>cdcl_twl_stgy_restart\<^sup>*\<^sup>* (S, 0, \<not>False) (W, n + 1, \<not>False)\<close> and
-    cdcl_twl_stgy_restart_with_leftovers_after_restart:
-      \<open>cdcl_twl_stgy_restart_with_leftovers (S, 0, \<not>False) (size (get_all_learned_clss W))
-        (W, n + 1, \<not>False)\<close> and
-    cdcl_twl_stgy_restart_with_leftovers_after_restart_T_V:
-    \<open>cdcl_twl_stgy_restart_with_leftovers (Ta, n, \<not>False) (size (get_all_learned_clss W))
-         (W, Suc n, \<not>False)\<close> and
-    cdcl_twl_stgy_restart_with_leftovers1_after_restart:
-      \<open>cdcl_twl_stgy_restart_with_leftovers1 (Ta, n, \<not>False) (W, Suc n, \<not>False)\<close>
-    if
-      f: \<open>True \<longrightarrow> f (snd (U, n)) < size (get_all_learned_clss (fst (U, n))) - m\<close> and
-      res: \<open>cdcl_twl_restart U V\<close> and
-      pre: \<open>cdcl_twl_stgy\<^sup>*\<^sup>* V W\<close> and
-      [unfolded brk, simp]: \<open>brk' = False\<close>
-    for V W
-  proof -
-    have \<open>S' \<noteq> U\<close>
-      using lits_to_update lits_to_upd_U by auto
-    then have \<open>cdcl_twl_o\<^sup>+\<^sup>+ S' U\<close>
-      using \<open>cdcl_twl_o\<^sup>*\<^sup>* S' U\<close> unfolding rtranclp_unfold by auto
-    then have st: \<open>cdcl_twl_stgy\<^sup>+\<^sup>+ Ta U\<close>
-      using TaT
-      by (meson local.cp rtranclp_cdcl_twl_cp_stgyD rtranclp_tranclp_tranclp
-          tranclp_cdcl_twl_o_stgyD)
-
-    show twl_res_T_V[unfolded not_False_eq_True]:
-      \<open>cdcl_twl_stgy_restart (Ta, n, \<not>False) (W, Suc n, \<not>False)\<close>
-      unfolding not_False_eq_True
-      apply (rule cdcl_twl_stgy_restart.restart_step[of _ U _ V])
-      subgoal by (rule st)
-      subgoal using f unfolding m by simp
-      subgoal by (rule res)
-      subgoal using pre by simp
-      done
-    show \<open>cdcl_twl_stgy_restart_with_leftovers (Ta, n, \<not>False)
-        (size (get_all_learned_clss W)) (W, Suc n, \<not>False)\<close>
-      unfolding not_False_eq_True cdcl_twl_stgy_restart_with_leftovers_def
-      by (rule exI[of _ \<open>W\<close>])(auto simp: twl_res_T_V)
-    show \<open>cdcl_twl_stgy_restart\<^sup>*\<^sup>* (S, 0, \<not>False) (W, n + 1, \<not>False)\<close>
-      using twl_res twl_res_T_V STa
-      unfolding cdcl_twl_stgy_restart_with_leftovers_def apply -
-      by (auto dest: cdcl_twl_stgy_restart_cdcl_twl_stgy_cdcl_twl_stgy_restart)
-    then show  \<open>cdcl_twl_stgy_restart_with_leftovers (S, 0, \<not>False) (size (get_all_learned_clss W))
-        (W, n + 1, \<not>False)\<close>
-      unfolding cdcl_twl_stgy_restart_with_leftovers_def apply -
-      by (rule exI[of _ W]) auto
-    show \<open>cdcl_twl_stgy_restart_with_leftovers1 (Ta, n, \<not>False) (W, Suc n, \<not>False)\<close>
-      using twl_res_T_V
-      unfolding cdcl_twl_stgy_restart_with_leftovers1_def not_False_eq_True
-      by fast
-  qed
-  let ?m = \<open>\<lambda>W. (size (get_all_learned_clss W))\<close>
-  have
-    twl_restart_after_restart_only:
-      \<open>cdcl_twl_stgy_restart (Ta, n, \<not>False) (V, n, \<not>False)\<close> and
-    rtranclp_twl_restart_after_restart_only:
-      \<open>cdcl_twl_stgy_restart\<^sup>*\<^sup>* (S, 0, \<not>False) (V, n, \<not>False)\<close> and
-    cdcl_twl_stgy_restart_with_leftovers_after_restart_only:
-      \<open>cdcl_twl_stgy_restart_with_leftovers (S, 0, \<not>False) (?m V) (V, n, \<not>False)\<close> and
-    cdcl_twl_stgy_restart_with_leftovers_after_restart_T_V:
-      \<open>cdcl_twl_stgy_restart_with_leftovers (Ta, n, \<not>False) (?m V) (V, n, \<not>False)\<close> and
-    cdcl_twl_stgy_restart_with_leftovers1_after_restart_only:
-    \<open>cdcl_twl_stgy_restart_with_leftovers1 (Ta, n, \<not>False) (V, n, \<not>False)\<close>
-    if
-      f: \<open>True \<longrightarrow> m < size (get_all_learned_clss U)\<close> and
-      res: \<open>cdcl_twl_restart_only U V\<close> and
-      [unfolded brk, simp]: \<open>brk' = False\<close>
-    for V
-  proof -
-    have \<open>S' \<noteq> U\<close>
-      using lits_to_update lits_to_upd_U by auto
-    then have \<open>cdcl_twl_o\<^sup>+\<^sup>+ S' U\<close>
-      using \<open>cdcl_twl_o\<^sup>*\<^sup>* S' U\<close> unfolding rtranclp_unfold by auto
-    then have st: \<open>cdcl_twl_stgy\<^sup>+\<^sup>+ Ta U\<close> and st2: \<open>cdcl_twl_stgy\<^sup>+\<^sup>+ T U\<close>
-      using TaT
-      by (meson local.cp rtranclp_cdcl_twl_cp_stgyD rtranclp_tranclp_tranclp
-          tranclp_cdcl_twl_o_stgyD)+
-
-    show twl_res_T_V[unfolded not_False_eq_True]:
-      \<open>cdcl_twl_stgy_restart (Ta, n, \<not>False) (V, n, \<not>False)\<close>
-      unfolding not_False_eq_True
-      apply (rule cdcl_twl_stgy_restart.restart_noGC[of _ U])
-      subgoal by (rule st)
-      subgoal using f unfolding m by simp
-      subgoal by (rule res)
-      done
-    show \<open>cdcl_twl_stgy_restart_with_leftovers (Ta, n, \<not>False) (?m V) (V, n, \<not>False)\<close>
-      unfolding not_False_eq_True cdcl_twl_stgy_restart_with_leftovers_def
-      by (rule exI[of _ \<open>V\<close>])(auto simp: twl_res_T_V)
-    show \<open>cdcl_twl_stgy_restart\<^sup>*\<^sup>* (S, 0, \<not>False) (V, n, \<not>False)\<close>
-      using twl_res twl_res_T_V TaT STa
-      unfolding cdcl_twl_stgy_restart_with_leftovers_def apply -
-      by auto
-    then show  \<open>cdcl_twl_stgy_restart_with_leftovers (S, 0, \<not>False) (?m V) (V, n, \<not>False)\<close>
-      unfolding cdcl_twl_stgy_restart_with_leftovers_def apply -
-      by (rule exI[of _ V]) auto
-    show \<open>cdcl_twl_stgy_restart_with_leftovers1 (Ta, n, \<not>False) (V, n, \<not>False)\<close>
-      using twl_res_T_V
-      unfolding cdcl_twl_stgy_restart_with_leftovers1_def not_False_eq_True
-      by fast
-  qed
-
-  have
-    rtranclp_twl_restart_after_restart_S_U:
-      \<open>cdcl_twl_stgy_restart_with_leftovers (S, 0, True) m (U, n, True)\<close> and
-    rtranclp_twl_restart_after_restart_T_U:
-      \<open>cdcl_twl_stgy_restart_with_leftovers (Ta, n, True) m (U, n, True)\<close>
-  proof -
-    have TaU: \<open>cdcl_twl_stgy\<^sup>*\<^sup>* Ta (fst (U, n))\<close>
-      using TaT \<open>cdcl_twl_stgy\<^sup>*\<^sup>* T U\<close> by auto
-    then show \<open>cdcl_twl_stgy_restart_with_leftovers (S, 0, True) m (U, n, True)\<close>
-      using STa m unfolding cdcl_twl_stgy_restart_with_leftovers_def
-      by fastforce
-    show \<open>cdcl_twl_stgy_restart_with_leftovers (Ta, n, True) m (U, n, True)\<close>
-      using \<open>cdcl_twl_stgy\<^sup>*\<^sup>* T U\<close> TaU m unfolding cdcl_twl_stgy_restart_with_leftovers_def
-      by fastforce
-  qed
-  have
-    rtranclp_twl_restart_after_restart_brk:
-      \<open>cdcl_twl_stgy_restart_with_leftovers (S, 0, True) m (U, n, True)\<close>
-    if
-      [simp]: \<open>brk = True\<close>
-  proof -
-    have \<open>full cdcl_twl_stgy T U \<or> get_conflict U \<noteq> None\<close>
-      using brk'_no_step \<open>cdcl_twl_stgy\<^sup>*\<^sup>* T U\<close>
-      unfolding rtranclp_unfold full_def final_twl_state_def by auto
-    then have \<open>(cdcl_twl_stgy\<^sup>*\<^sup>* T U \<and> pcdcl_twl_final_state U) \<or> get_conflict U \<noteq> None\<close>
-      unfolding full_def pcdcl_twl_final_state_def
-      by auto
-    then consider
-        (step) \<open>cdcl_twl_stgy_restart (T, n, True) (U, n, False)\<close> |
-        (final) \<open>get_conflict U \<noteq> None\<close>
-      using cdcl_twl_stgy_restart.intros(3)[of T U]
-      by (auto dest!: cdcl_twl_stgy_restart.intros)
-    then show \<open>cdcl_twl_stgy_restart_with_leftovers (S, 0, True) m (U, n, True)\<close>
-    proof cases
-      case step
-      then show ?thesis
-        using twl_res \<open>cdcl_twl_stgy\<^sup>*\<^sup>* T U\<close> unfolding cdcl_twl_stgy_restart_with_leftovers_def
-        using cdcl_twl_stgy_restart_cdcl_twl_stgy_cdcl_twl_stgy_restart2[of T n True U] apply -
-        by fastforce
-    next
-      case final
-      then show ?thesis
-        using twl_res \<open>cdcl_twl_stgy\<^sup>*\<^sup>* T U\<close>  unfolding cdcl_twl_stgy_restart_with_leftovers_def
-        by fastforce
-    qed
-  qed
-  have cdcl_twl_stgy_restart_with_leftovers1_T_U:
-    \<open>cdcl_twl_stgy_restart_with_leftovers1 (T, n, True) (U, n, True) \<longleftrightarrow> T \<noteq> U\<close>
-  proof -
-    have \<open>cdcl_twl_stgy\<^sup>+\<^sup>+ T U \<or> T = U\<close>
-      using \<open>cdcl_twl_stgy\<^sup>*\<^sup>* T U\<close> unfolding rtranclp_unfold by auto
-    then show ?thesis
-      using wf_not_refl[OF wf_cdcl_twl_stgy_restart, of \<open>(U, n, True)\<close>]
-      using wf_not_refl[OF tranclp_wf_cdcl_twl_stgy, of \<open>U\<close>]
-        struct_invs_U
-      unfolding cdcl_twl_stgy_restart_with_leftovers1_def by auto
-  qed
-  have brk'_eq: \<open>\<not>cdcl_twl_stgy_restart_with_leftovers1 (T, n, True) (U, n, True) \<Longrightarrow> brk'\<close>
-    using cdcl_o lits_to_upd_U lits_to_update local.cp
-    unfolding cdcl_twl_stgy_restart_with_leftovers1_def
-    unfolding rtranclp_unfold
-    by (auto dest!: tranclp_cdcl_twl_o_stgyD tranclp_cdcl_twl_cp_stgyD
-        simp: rtranclp_unfold
-        dest: rtranclp_tranclp_tranclp tranclp_trans)
-
-  have [simp]: \<open>brk = False\<close>
-    using cond by auto
-  show ?A
-    unfolding restart_prog_def restart_required_def
-    apply (refine_vcg; remove_dummy_vars)
-    subgoal using struct_invs_U stgy_invs_U confl_U unfolding restart_prog_pre_def by fast
-    subgoal using cdcl_twl_restart_only_twl_struct_invs struct_invs_U by blast
-    subgoal using cdcl_twl_stgy_restart_only_twl_stgy_invs stgy_invs_U by blast
-    subgoal by simp
-    subgoal by (rule cdcl_twl_stgy_restart_with_leftovers_after_restart_only)
-    subgoal by (auto simp add: cdcl_twl_restart_only.simps)
-    subgoal by (auto simp add: cdcl_twl_restart_only.simps)
-    subgoal apply (auto intro!: struct_invs_S struct_invs_T
-      cdcl_twl_stgy_restart_with_leftovers1_after_restart_only[unfolded not_False_eq_True])
-thm 
-  cdcl_twl_stgy_restart_with_leftovers1_after_restart_only[unfolded not_False_eq_True]
-
-      apply (rule 
-        cdcl_twl_stgy_restart_with_leftovers1_after_restart_only[unfolded not_False_eq_True])
-      sorry
-    subgoal by (rule struct_invs')
-    subgoal by (rule stgy_invs)
-    subgoal by simp
-    subgoal
-      by (rule cdcl_twl_stgy_restart_with_leftovers_after_restart, simp)
-    subgoal
-      using rtranclp_twl_restart_after_restart_T_U
-      by (auto intro!: struct_invs_S struct_invs_T
-        cdcl_twl_stgy_restart_with_leftovers1_after_restart[unfolded not_False_eq_True])
-    subgoal by (rule struct_invs_U)
-    subgoal by (rule stgy_invs_U)
-    subgoal by (rule brk'_no_step) simp
-    subgoal
-      by (auto intro: rtranclp_twl_restart_after_restart_brk
-        rtranclp_twl_restart_after_restart_S_U)
-    subgoal by (rule clss_to_upd_U)
-    subgoal using struct_invs_U conflict_U lits_to_upd_U
-      by (cases \<open>get_conflict U\<close>)(auto simp: twl_struct_invs_def)
-    subgoal
-      using cdcl_twl_stgy_restart_with_leftovers1_T_U brk'_eq
-      by (auto simp: twl_restart_after_restart struct_invs_S struct_invs_T
-        cdcl_twl_stgy_restart_with_leftovers_after_restart_T_V struct_invs_U
-        rtranclp_twl_restart_after_restart_brk rtranclp_twl_restart_after_restart_T_U
-        cdcl_twl_stgy_restart_with_leftovers1_after_restart)
+      by (rule restart_prog_spec)
+    subgoal for init_ebrk brkT T' m n ebrk T
+      by (rule_tac x=T' in exI) (auto simp: cdcl_twl_stgy_restart_prog_inv_def)
     done
 qed
 
-lemma (in twl_restart)
-  assumes
-    inv: \<open>case (ebrk, brk, T, m, n) of  (ebrk, brk, T, m, n) \<Rightarrow> cdcl_twl_stgy_restart_prog_inv S brk T m n\<close> and
-    cond: \<open>case (ebrk, brk, T, m, n) of (ebrk, brk, _) \<Rightarrow> \<not> brk \<and> \<not>ebrk\<close> and
-    other_inv: \<open>cdcl_twl_o_prog_spec S' (brk', U)\<close> and
-    struct_invs_S: \<open>twl_struct_invs S'\<close> and
-    cp: \<open>cdcl_twl_cp\<^sup>*\<^sup>* T S'\<close> and
-    lits_to_update: \<open>literals_to_update S' = {#}\<close> and
-    \<open>\<forall>S'a. \<not> cdcl_twl_cp S' S'a\<close> and
-    \<open>twl_stgy_invs S'\<close> and
-    brk: \<open>(brk', brk) \<in> bool_rel\<close>
-  shows restart_prog_early_spec:
-   \<open>restart_prog U m n brk'
-    \<le> SPEC (\<lambda>x. (case x of (T, m, n) \<Rightarrow> RES UNIV \<bind> (\<lambda>ebrk. RETURN (ebrk, brk', T, m, n)))
-            \<le> SPEC
-               (\<lambda>s'. (case s' of (ebrk, brk, x, xb, xc) \<Rightarrow>
-                        cdcl_twl_stgy_restart_prog_inv S brk x xb xc) \<and>
-                     (s', ebrk, brk, T, n)
-                     \<in> {((ebrk, brkT, T, m, n'), ebrk, brkS, S, _).
-                        twl_struct_invs S \<and>
-                        cdcl_twl_stgy_restart_with_leftovers1 (S, n, \<not>brkT) (T, n', \<not>brkS)} \<union>
-                       {((ebrkT, brkT, T, m), ebrkS, brkS, S, n).
-                           S = T \<and> (ebrkT \<or> brkT) \<and> \<not> brkS \<and> \<not> ebrkS}))\<close>  (is \<open>?B\<close>)
-proof -
-  have brk[simp]: \<open>brk' = brk\<close>
-    using brk by auto
-  have struct_invs': \<open>cdcl_twl_restart U T \<Longrightarrow> cdcl_twl_stgy\<^sup>*\<^sup>* T V \<Longrightarrow> twl_struct_invs V\<close> for T V
-    using assms(3) cdcl_twl_restart_twl_struct_invs
-    by (metis (no_types, lifting) case_prodD rtranclp_cdcl_twl_stgy_twl_struct_invs)
-  have stgy_invs: \<open>cdcl_twl_restart U V \<Longrightarrow> cdcl_twl_stgy\<^sup>*\<^sup>* V W \<Longrightarrow> twl_stgy_invs W\<close> for V W
-    using assms(3) cdcl_twl_restart_twl_stgy_invs
-    by (metis (no_types, lifting) case_prodD cdcl_twl_restart_twl_struct_invs
-      rtranclp_cdcl_twl_stgy_twl_stgy_invs)
-  have res_no_clss_to_upd: \<open>cdcl_twl_restart U V \<Longrightarrow> clauses_to_update V = {#}\<close> for V
-    by (auto simp: cdcl_twl_restart.simps)
-  have res_no_confl: \<open>cdcl_twl_restart U V \<Longrightarrow> get_conflict V = None\<close> for V
-    by (auto simp: cdcl_twl_restart.simps)
 
-  have
-    struct_invs_T: \<open>twl_struct_invs T\<close> and
-    \<open>twl_stgy_invs T\<close> and
-    \<open>brk \<longrightarrow> final_twl_state T\<close> and
-    twl_res: \<open>cdcl_twl_stgy_restart_with_leftovers (S, 0, True) m (T, n, True)\<close> and
-    \<open>clauses_to_update T = {#}\<close> and
-    confl: \<open>\<not> brk \<longrightarrow> get_conflict T = None\<close>
-    using inv unfolding cdcl_twl_stgy_restart_prog_inv_def by fast+
-
-  have
-    cdcl_o: \<open>cdcl_twl_o\<^sup>*\<^sup>* S' U\<close> and
-    conflict_U: \<open>get_conflict U \<noteq> None \<Longrightarrow> count_decided (get_trail U) = 0\<close> and
-    brk'_no_step: \<open>brk' \<Longrightarrow> final_twl_state U\<close> and
-    struct_invs_U: \<open>twl_struct_invs U\<close> and
-    stgy_invs_U: \<open>twl_stgy_invs U\<close> and
-    clss_to_upd_U: \<open>clauses_to_update U = {#}\<close> and
-    lits_to_upd_U: \<open>\<not> brk' \<longrightarrow> literals_to_update U \<noteq> {#}\<close> and
-    confl_U: \<open>\<not> brk' \<longrightarrow> get_conflict U = None\<close>
-    using other_inv unfolding final_twl_state_def by fast+
-
-  have \<open>cdcl_twl_stgy\<^sup>*\<^sup>* T U\<close>
-    by (meson \<open>cdcl_twl_o\<^sup>*\<^sup>* S' U\<close> assms(5) rtranclp_cdcl_twl_cp_stgyD rtranclp_cdcl_twl_o_stgyD
-        rtranclp_trans)
-  from twl_res obtain Ta where
-    STa: \<open>cdcl_twl_stgy_restart\<^sup>*\<^sup>* (S, 0, True) (Ta, n, True)\<close> and
-    TaT: \<open>cdcl_twl_stgy\<^sup>*\<^sup>* Ta T\<close> and
-    m: \<open>m = size (get_all_learned_clss Ta)\<close>
-    unfolding cdcl_twl_stgy_restart_with_leftovers_def prod.case snd_conv fst_conv
-    by blast
-
-  let ?m = \<open>\<lambda>W. (size (get_all_learned_clss W))\<close>
-  have
-    twl_restart_after_restart:
-      \<open>cdcl_twl_stgy_restart (Ta, n, True) (W, Suc n, True)\<close> and
-    rtranclp_twl_restart_after_restart:
-      \<open>cdcl_twl_stgy_restart\<^sup>*\<^sup>* (S, 0, True) (W, n + 1, True)\<close> and
-    cdcl_twl_stgy_restart_with_leftovers_after_restart:
-      \<open>cdcl_twl_stgy_restart_with_leftovers (S, 0, True) (?m W) (W, n + 1, True)\<close> and
-    cdcl_twl_stgy_restart_with_leftovers_after_restart_T_W:
-      \<open>cdcl_twl_stgy_restart_with_leftovers (Ta, n, True) (?m W) (W, Suc n, True)\<close> and
-    cdcl_twl_stgy_restart_with_leftovers1_after_restart:
-      \<open>cdcl_twl_stgy_restart_with_leftovers1 (Ta, n, True) (W, Suc n, True)\<close>
-    if
-      f: \<open>True \<longrightarrow> f (snd (U, n)) < size (get_all_learned_clss (fst (U, n))) - m\<close> and
-      res: \<open>cdcl_twl_restart U V\<close> and
-      inp: \<open>cdcl_twl_stgy\<^sup>*\<^sup>* V W\<close> and
-      [unfolded brk, simp]: \<open>brk' = False\<close>
-    for V W
-  proof -
-    have \<open>S' \<noteq> U\<close>
-      using lits_to_update lits_to_upd_U by auto
-    then have \<open>cdcl_twl_o\<^sup>+\<^sup>+ S' U\<close>
-      using \<open>cdcl_twl_o\<^sup>*\<^sup>* S' U\<close> unfolding rtranclp_unfold by auto
-    then have st: \<open>cdcl_twl_stgy\<^sup>+\<^sup>+ Ta U\<close> and st': \<open>cdcl_twl_stgy\<^sup>+\<^sup>+ T U\<close>
-      using TaT
-      by (meson local.cp rtranclp_cdcl_twl_cp_stgyD rtranclp_tranclp_tranclp
-          tranclp_cdcl_twl_o_stgyD)+
-
-    show twl_res_T_V: \<open>cdcl_twl_stgy_restart (Ta, n, True) (W, Suc n, True)\<close>
-      apply (rule cdcl_twl_stgy_restart.restart_step[of _ U _ V])
-      subgoal by (rule st)
-      subgoal using f unfolding m by simp
-      subgoal by (rule res)
-      subgoal by (rule inp)
-      done
-    show \<open>cdcl_twl_stgy_restart_with_leftovers (Ta, n, True) (?m W) (W, Suc n, True)\<close>
-      unfolding cdcl_twl_stgy_restart_with_leftovers_def
-      by (rule exI[of _ \<open>W\<close>])(auto simp: twl_res_T_V)
-    show \<open>cdcl_twl_stgy_restart\<^sup>*\<^sup>* (S, 0, True) (W, n + 1, True)\<close>
-      using twl_res twl_res_T_V STa
-      unfolding cdcl_twl_stgy_restart_with_leftovers_def apply -
-      by (auto dest: cdcl_twl_stgy_restart_cdcl_twl_stgy_cdcl_twl_stgy_restart)
-    then show  \<open>cdcl_twl_stgy_restart_with_leftovers (S, 0, True) (?m W) (W, n + 1, True)\<close>
-      unfolding cdcl_twl_stgy_restart_with_leftovers_def apply -
-      by (rule exI[of _ W]) auto
-    show \<open>cdcl_twl_stgy_restart_with_leftovers1 (Ta, n, True) (W, Suc n, True)\<close>
-      using twl_res_T_V
-      unfolding cdcl_twl_stgy_restart_with_leftovers1_def
-      by fast
-  qed
-  have
-    twl_restart_after_restart_only:
-      \<open>cdcl_twl_stgy_restart (Ta, n, \<not>False) (V, n, \<not>False)\<close> and
-    rtranclp_twl_restart_after_restart_only:
-      \<open>cdcl_twl_stgy_restart\<^sup>*\<^sup>* (S, 0, \<not>False) (V, n, \<not>False)\<close> and
-    cdcl_twl_stgy_restart_with_leftovers_after_restart_only:
-      \<open>cdcl_twl_stgy_restart_with_leftovers (S, 0, \<not>False) (?m V) (V, n, \<not>False)\<close> and
-    cdcl_twl_stgy_restart_with_leftovers_after_restart_T_V:
-      \<open>cdcl_twl_stgy_restart_with_leftovers (Ta, n, \<not>False) (?m V) (V, n, \<not>False)\<close> and
-    cdcl_twl_stgy_restart_with_leftovers1_after_restart_only:
-      \<open>cdcl_twl_stgy_restart_with_leftovers1 (Ta, n, \<not>False) (V, n, \<not>False)\<close>
-    if
-      f: \<open>True \<longrightarrow> m < size (get_all_learned_clss U)\<close> and
-      res: \<open>cdcl_twl_restart_only U V\<close> and
-      [unfolded brk, simp]: \<open>brk' = False\<close>
-    for V
-  proof -
-    have \<open>S' \<noteq> U\<close>
-      using lits_to_update lits_to_upd_U by auto
-    then have \<open>cdcl_twl_o\<^sup>+\<^sup>+ S' U\<close>
-      using \<open>cdcl_twl_o\<^sup>*\<^sup>* S' U\<close> unfolding rtranclp_unfold by auto
-    then have st: \<open>cdcl_twl_stgy\<^sup>+\<^sup>+ Ta U\<close> and st2: \<open>cdcl_twl_stgy\<^sup>+\<^sup>+ T U\<close>
-      using TaT
-      by (meson local.cp rtranclp_cdcl_twl_cp_stgyD rtranclp_tranclp_tranclp
-          tranclp_cdcl_twl_o_stgyD)+
-
-    show twl_res_T_V[unfolded not_False_eq_True]:
-      \<open>cdcl_twl_stgy_restart (Ta, n, \<not>False) (V, n, \<not>False)\<close>
-      unfolding not_False_eq_True
-      apply (rule cdcl_twl_stgy_restart.restart_noGC[of _ U])
-      subgoal by (rule st)
-      subgoal using f unfolding m by simp
-      subgoal by (rule res)
-      done
-    show \<open>cdcl_twl_stgy_restart_with_leftovers (Ta, n, \<not>False) (?m V) (V, n, \<not>False)\<close>
-      unfolding not_False_eq_True cdcl_twl_stgy_restart_with_leftovers_def
-      by (rule exI[of _ \<open>V\<close>])(auto simp: twl_res_T_V)
-    show \<open>cdcl_twl_stgy_restart\<^sup>*\<^sup>* (S, 0, \<not>False) (V, n, \<not>False)\<close>
-      using twl_res twl_res_T_V TaT STa
-      unfolding cdcl_twl_stgy_restart_with_leftovers_def apply -
-      by auto
-    then show  \<open>cdcl_twl_stgy_restart_with_leftovers (S, 0, \<not>False) (?m V) (V, n, \<not>False)\<close>
-      unfolding cdcl_twl_stgy_restart_with_leftovers_def apply -
-      by (rule exI[of _ V]) auto
-    show \<open>cdcl_twl_stgy_restart_with_leftovers1 (Ta, n, \<not>False) (V, n, \<not>False)\<close>
-      using twl_res_T_V
-      unfolding cdcl_twl_stgy_restart_with_leftovers1_def not_False_eq_True
-      by fast
-  qed
-  have
-    rtranclp_twl_restart_after_restart_S_U:
-      \<open>cdcl_twl_stgy_restart_with_leftovers (S, 0, True) m (U, n, True)\<close> and
-    rtranclp_twl_restart_after_restart_T_U:
-      \<open>cdcl_twl_stgy_restart_with_leftovers (Ta, n, True) m (U, n, True)\<close>
-  proof -
-    have TaU: \<open>cdcl_twl_stgy\<^sup>*\<^sup>* Ta (fst (U, n))\<close>
-      using TaT \<open>cdcl_twl_stgy\<^sup>*\<^sup>* T U\<close> by auto
-    then show \<open>cdcl_twl_stgy_restart_with_leftovers (S, 0, True) m (U, n, True)\<close>
-      using STa m unfolding cdcl_twl_stgy_restart_with_leftovers_def
-      by fastforce
-    show \<open>cdcl_twl_stgy_restart_with_leftovers (Ta, n, True) m (U, n, True)\<close>
-      using \<open>cdcl_twl_stgy\<^sup>*\<^sup>* T U\<close> TaU m unfolding cdcl_twl_stgy_restart_with_leftovers_def
-      by fastforce
-  qed
-  have
-    rtranclp_twl_restart_after_restart_brk:
-      \<open>cdcl_twl_stgy_restart_with_leftovers (S, 0, True) m (U, n, True)\<close>
-    if
-      [simp]: \<open>brk = True\<close>
-  proof -
-    have \<open>full cdcl_twl_stgy T U \<or> get_conflict U \<noteq> None\<close>
-      using brk'_no_step \<open>cdcl_twl_stgy\<^sup>*\<^sup>* T U\<close>
-      unfolding rtranclp_unfold full_def final_twl_state_def by auto
-    then have \<open>(cdcl_twl_stgy\<^sup>*\<^sup>* T U \<and> pcdcl_twl_final_state U) \<or> get_conflict U \<noteq> None\<close>
-      unfolding full_def pcdcl_twl_final_state_def
-      by auto
-    then consider
-        (step) \<open>cdcl_twl_stgy_restart (T, n, True) (U, n, False)\<close> |
-        (final) \<open>get_conflict U \<noteq> None\<close>
-      using cdcl_twl_stgy_restart.intros(3)[of T U]
-      by (auto dest!: cdcl_twl_stgy_restart.intros)
-    then show \<open>cdcl_twl_stgy_restart_with_leftovers (S, 0, True) m (U, n, True)\<close>
-    proof cases
-      case step
-      then show ?thesis
-        using twl_res \<open>cdcl_twl_stgy\<^sup>*\<^sup>* T U\<close> unfolding cdcl_twl_stgy_restart_with_leftovers_def
-        using cdcl_twl_stgy_restart_cdcl_twl_stgy_cdcl_twl_stgy_restart2[of T n True U] apply -
-        by fastforce
-    next
-      case final
-      then show ?thesis
-        using twl_res \<open>cdcl_twl_stgy\<^sup>*\<^sup>* T U\<close>  unfolding cdcl_twl_stgy_restart_with_leftovers_def
-        by fastforce
-    qed
-  qed
-  have cdcl_twl_stgy_restart_with_leftovers1_T_U:
-    \<open>cdcl_twl_stgy_restart_with_leftovers1 (T, n, True) (U, n, True) \<longleftrightarrow> T \<noteq> U\<close>
-  proof -
-    have \<open>cdcl_twl_stgy\<^sup>+\<^sup>+ T U \<or> T = U\<close>
-      using \<open>cdcl_twl_stgy\<^sup>*\<^sup>* T U\<close> unfolding rtranclp_unfold by auto
-    then show ?thesis
-      using wf_not_refl[OF wf_cdcl_twl_stgy_restart, of \<open>(U, n, True)\<close>]
-      using wf_not_refl[OF tranclp_wf_cdcl_twl_stgy, of \<open>U\<close>]
-        struct_invs_U
-      unfolding cdcl_twl_stgy_restart_with_leftovers1_def by auto
-  qed
-  have brk'_eq: \<open>\<not>cdcl_twl_stgy_restart_with_leftovers1 (T, n, True) (U, n, True) \<Longrightarrow> brk'\<close>
-    using cdcl_o lits_to_upd_U lits_to_update local.cp
-    unfolding cdcl_twl_stgy_restart_with_leftovers1_def
-    unfolding rtranclp_unfold
-    by (auto dest!: tranclp_cdcl_twl_o_stgyD tranclp_cdcl_twl_cp_stgyD
-        simp: rtranclp_unfold
-        dest: rtranclp_tranclp_tranclp tranclp_trans)
-
-  have H[simp]: \<open>brk = False\<close>
-    using cond by auto
-  show ?B
-    unfolding restart_prog_def restart_required_def
-    apply (refine_vcg; remove_dummy_vars)
-    subgoal using struct_invs_U stgy_invs_U confl_U unfolding restart_prog_pre_def by fast
-    subgoal
-      unfolding cdcl_twl_stgy_restart_prog_inv_def
-      apply (intro conjI)
-      subgoal using cdcl_twl_restart_only_twl_struct_invs struct_invs_U by blast
-      subgoal using cdcl_twl_stgy_restart_only_twl_stgy_invs stgy_invs_U by blast
-      subgoal by simp
-      subgoal by (rule cdcl_twl_stgy_restart_with_leftovers_after_restart_only[unfolded not_False_eq_True]) simp_all
-      subgoal by (auto simp: cdcl_twl_restart_only.simps)
-      subgoal by (auto simp: cdcl_twl_restart_only.simps)
-      done
-    subgoal
-      using rtranclp_twl_restart_after_restart_T_U
-      by (auto intro!: struct_invs_S struct_invs_T
-        cdcl_twl_stgy_restart_with_leftovers1_after_restart_only[unfolded not_False_eq_True])
-    subgoal
-      unfolding cdcl_twl_stgy_restart_prog_inv_def
-      apply (intro conjI)
-      subgoal by (rule struct_invs')
-      subgoal by (rule stgy_invs)
-      subgoal unfolding H by fast
-      subgoal by (rule cdcl_twl_stgy_restart_with_leftovers_after_restart) simp_all
-      subgoal by simp
-      subgoal by (simp add: res_no_confl)
-      done
-    subgoal
-      using cdcl_twl_stgy_restart_with_leftovers1_T_U brk'_eq
-      by (auto simp: twl_restart_after_restart struct_invs_S struct_invs_T
-        cdcl_twl_stgy_restart_with_leftovers_after_restart_T_W struct_invs_U
-        rtranclp_twl_restart_after_restart_brk rtranclp_twl_restart_after_restart_T_U
-        cdcl_twl_stgy_restart_with_leftovers1_after_restart)
-    subgoal
-      using inv
-      unfolding cdcl_twl_stgy_restart_prog_inv_def
-      by (simp add: struct_invs_U stgy_invs_U clss_to_upd_U lits_to_upd_U
-        confl_U rtranclp_twl_restart_after_restart_S_U)
-    subgoal
-      using inv cdcl_twl_stgy_restart_with_leftovers1_T_U H brk brk'_eq
-      unfolding cdcl_twl_stgy_restart_prog_inv_def
-      apply (simp add: struct_invs_U stgy_invs_U clss_to_upd_U lits_to_upd_U
-        confl_U rtranclp_twl_restart_after_restart_S_U)
-      by auto
-    done
-qed
-
-lemma cdcl_twl_stgy_restart_with_leftovers_refl:
-  \<open>cdcl_twl_stgy_restart_with_leftovers (S, a) (size (get_all_learned_clss S)) (S, a)\<close>
-  unfolding cdcl_twl_stgy_restart_with_leftovers_def
-  by (rule exI[of _ \<open>S\<close>]) auto
-
-(* declare restart_prog_spec[THEN order_trans, refine_vcg] 
-lemma (in twl_restart) cdcl_twl_stgy_restart_prog_spec:
+lemma cdcl_twl_stgy_restart_prog_spec:
+  fixes S :: \<open>'v twl_st\<close>
   assumes \<open>twl_struct_invs S\<close> and \<open>twl_stgy_invs S\<close> and \<open>clauses_to_update S = {#}\<close> and
     \<open>get_conflict S = None\<close>
   shows
     \<open>cdcl_twl_stgy_restart_prog S \<le> SPEC(\<lambda>T.
-       \<exists>m n. cdcl_twl_stgy_restart_with_leftovers (S, 0, True) m (T, n, True) \<and>
+       \<exists>S' m n. cdcl_twl_stgy_restart_with_leftovers (S, 0, True) m S' (T, n, True) \<and>
         final_twl_state T)\<close>
     (is \<open>_ \<le> SPEC(\<lambda>T. ?P T)\<close>)
 proof -
-  have final_prop: \<open>?P T\<close>
-    if
-     inv: \<open>case (brk, T, n) of  (brk, T, m, n) \<Rightarrow> cdcl_twl_stgy_restart_prog_inv S brk T m n\<close> and
-      \<open>\<not> (case (brk, T, n) of (brk, uu_) \<Rightarrow> \<not> brk)\<close>
-    for brk T n
-  proof -
-    have
-      \<open>brk\<close> and
-      \<open>twl_struct_invs T\<close> and
-      \<open>twl_stgy_invs T\<close> and
-      ns: \<open>final_twl_state T\<close> and
-      twl_left_overs: \<open>cdcl_twl_stgy_restart_with_leftovers (S, 0) (T, n)\<close> and
-      \<open>clauses_to_update T = {#}\<close>
-      using that unfolding cdcl_twl_stgy_restart_prog_inv_def by auto
-    obtain S' where
-       st: \<open>cdcl_twl_stgy_restart\<^sup>*\<^sup>* (S, 0) (S', n)\<close> and
-       S'_T: \<open>cdcl_twl_stgy\<^sup>*\<^sup>* S' T\<close>
-      using twl_left_overs unfolding cdcl_twl_stgy_restart_with_leftovers_def by auto
-    then show ?thesis
-      using ns unfolding cdcl_twl_stgy_restart_with_leftovers_def apply -
-      apply (rule_tac x=n in exI)
-      apply (rule conjI)
-      subgoal by (rule_tac x=S' in exI) auto
-      subgoal by auto
-      done
-  qed
-  show ?thesis
-    supply RETURN_as_SPEC_refine[refine2 del]
-    unfolding cdcl_twl_stgy_restart_prog_def full_def cdcl_twl_stgy_restart_prog_inv_def
-    apply (refine_vcg WHILEIT_rule[where
-           R = \<open>{((brkT, T, n), (brkS, S, m)).
-                     twl_struct_invs S \<and> cdcl_twl_stgy_restart_with_leftovers1 (S, m) (T, n)} \<union>
-                {((brkT, T), (brkS, S)). S = T \<and> brkT \<and> \<not>brkS}\<close>];
-        remove_dummy_vars)
-    subgoal by (rule wf_cdcl_twl_stgy_restart_measure)
-    subgoal using assms by fast
-    subgoal using assms by fast
-    subgoal using assms by fast
-    subgoal by (rule cdcl_twl_stgy_restart_with_leftovers_refl)
-    subgoal using assms by fast
-    subgoal using assms by fast
-    subgoal by fast
-    subgoal by fast
-    subgoal by fast
-    subgoal by fast
-    subgoal by (simp add: no_step_cdcl_twl_cp_no_step_cdcl\<^sub>W_cp)
-    subgoal by fast
-    subgoal by (rule restart_prog_spec[unfolded cdcl_twl_stgy_restart_prog_inv_def])
-    subgoal by (rule final_prop[unfolded cdcl_twl_stgy_restart_prog_inv_def])
-    done
-qed
-definition cdcl_twl_stgy_restart_prog_early :: "'v twl_st \<Rightarrow> 'v twl_st nres" where
-  \<open>cdcl_twl_stgy_restart_prog_early S\<^sub>0 =
-  do {
-    ebrk \<leftarrow> RES UNIV;
-    (ebrk, brk, T, n) \<leftarrow> WHILE\<^sub>T\<^bsup>\<lambda>(ebrk, brk, T, m, n). cdcl_twl_stgy_restart_prog_inv S\<^sub>0 brk T m n\<^esup>
-      (\<lambda>(ebrk, brk, _). \<not>brk \<and> \<not>ebrk)
-      (\<lambda>(ebrk, brk, S, n).
+  have cdcl_twl_stgy_restart_prog_alt_def:
+    \<open>cdcl_twl_stgy_restart_prog S\<^sub>0 =
+    do {
+    _ \<leftarrow> RETURN False;
+    (brk, _, T, _, _) \<leftarrow> WHILE\<^sub>T\<^bsup>cdcl_twl_stgy_restart_prog_inv S\<^sub>0\<^esup>
+      (\<lambda>(brk, _). \<not>brk)
+      (\<lambda>(brk, S, S', m, n).
       do {
-        T \<leftarrow> unit_propagation_outer_loop S;
+        T \<leftarrow> unit_propagation_outer_loop S';
         (brk, T) \<leftarrow> cdcl_twl_o_prog T;
-        (T, n) \<leftarrow> restart_prog T n brk;
-	ebrk \<leftarrow> RES UNIV;
-        RETURN (ebrk, brk, T, n)
+        (b, T, m', n') \<leftarrow> restart_prog T m n brk;
+        _ \<leftarrow> RETURN False;
+        RETURN (brk, if b then T else S, T, m', n')
       })
-      (ebrk, False, S\<^sub>0, 0);
-    if \<not>brk then do {
-      (brk, T, _) \<leftarrow> WHILE\<^sub>T\<^bsup>\<lambda>(brk, T, n). cdcl_twl_stgy_restart_prog_inv S\<^sub>0 brk T n\<^esup>
-	(\<lambda>(brk, _). \<not>brk)
-	(\<lambda>(brk, S, n).
-	do {
-	  T \<leftarrow> unit_propagation_outer_loop S;
-	  (brk, T) \<leftarrow> cdcl_twl_o_prog T;
-	  (T, n) \<leftarrow> restart_prog T n brk;
-	  RETURN (brk, T, n)
-	})
-	(False, T, n);
-      RETURN T
-    }
-    else RETURN T
-  }\<close>
+      (False, S\<^sub>0, S\<^sub>0, size (get_all_learned_clss S\<^sub>0), 0);
+    RETURN T
+    }\<close> for S\<^sub>0 :: \<open>'v twl_st\<close>
+    unfolding cdcl_twl_stgy_restart_prog_def
+    by auto
+  have [refine]: \<open>RETURN False \<le> \<Down> {(b, b'). (b = b') \<and> \<not>b} (RES UNIV)\<close>
+    by (auto intro!: RETURN_RES_refine)
+   have [refine]: \<open>((False, S, S, size (get_all_learned_clss S), (0 :: nat)), ebrk, False, S, S,
+     size (get_all_learned_clss S), 0) \<in> {(T, (b, S)). S = T \<and> \<not>b}\<close>
+     if \<open>(u, ebrk) \<in> {(b, b'). (b = b') \<and> \<not>b}\<close> for ebrk u
+     using that
+     by auto
+   have this_is_the_identity: \<open>x \<le> \<Down>Id (x')\<close> if \<open>x = x'\<close>
+     for x x'
+     using that by auto
 
-lemma (in twl_restart) cdcl_twl_stgy_prog_early_spec:
-  assumes \<open>twl_struct_invs S\<close> and \<open>twl_stgy_invs S\<close> and \<open>clauses_to_update S = {#}\<close> and
-    \<open>get_conflict S = None\<close>
-  shows
-    \<open>cdcl_twl_stgy_restart_prog_early S \<le> SPEC(\<lambda>T. \<exists>n. cdcl_twl_stgy_restart_with_leftovers (S, 0) (T, n) \<and>
-        final_twl_state T)\<close>
-    (is \<open>_ \<le> SPEC(\<lambda>T. ?P T)\<close>)
-proof -
-  have final_prop: \<open>?P T\<close>
-    if
-     inv: \<open>case (brk, T, n) of  (brk, T, m) \<Rightarrow> cdcl_twl_stgy_restart_prog_inv S brk T m\<close> and
-      \<open>\<not> (case (brk, T, n) of (brk, uu_) \<Rightarrow> \<not> brk)\<close>
-    for brk T n
-  proof -
-    have
-      \<open>brk\<close> and
-      \<open>twl_struct_invs T\<close> and
-      \<open>twl_stgy_invs T\<close> and
-      ns: \<open>final_twl_state T\<close> and
-      twl_left_overs: \<open>cdcl_twl_stgy_restart_with_leftovers (S, 0) (T, n)\<close> and
-      \<open>clauses_to_update T = {#}\<close>
-      using that unfolding cdcl_twl_stgy_restart_prog_inv_def by auto
-    obtain S' where
-       st: \<open>cdcl_twl_stgy_restart\<^sup>*\<^sup>* (S, 0) (S', n)\<close> and
-       S'_T: \<open>cdcl_twl_stgy\<^sup>*\<^sup>* S' T\<close>
-      using twl_left_overs unfolding cdcl_twl_stgy_restart_with_leftovers_def by auto
-    then show ?thesis
-      using ns unfolding cdcl_twl_stgy_restart_with_leftovers_def apply -
-      apply (rule_tac x=n in exI)
-      apply (rule conjI)
-      subgoal by (rule_tac x=S' in exI) auto
-      subgoal by auto
-      done
-  qed
-  show ?thesis
-    supply RETURN_as_SPEC_refine[refine2 del]
-    unfolding cdcl_twl_stgy_restart_prog_early_def full_def
-    apply (refine_vcg
-        WHILEIT_rule[where
-           R = \<open>{((ebrk, brkT, T, n), (ebrk, brkS, S, m)).
-                     twl_struct_invs S \<and> cdcl_twl_stgy_restart_with_leftovers1 (S, m) (T, n)} \<union>
-                {((ebrkT, brkT, T), (ebrkS, brkS, S)). S = T \<and> (ebrkT \<or> brkT) \<and> (\<not>brkS \<and> \<not>ebrkS)}\<close>]
-       WHILEIT_rule[where
-           R = \<open>{((brkT, T, n), (brkS, S, m)).
-                     twl_struct_invs S \<and> cdcl_twl_stgy_restart_with_leftovers1 (S, m) (T, n)} \<union>
-                {((brkT, T), (brkS, S)). S = T \<and> brkT \<and> \<not>brkS}\<close>];
-        remove_dummy_vars)
-    subgoal by (rule wf_cdcl_twl_stgy_restart_measure_early)
-    subgoal using assms unfolding cdcl_twl_stgy_restart_prog_inv_def
-      by (fast intro: cdcl_twl_stgy_restart_with_leftovers_refl)
-    subgoal unfolding cdcl_twl_stgy_restart_prog_inv_def by fast
-    subgoal unfolding cdcl_twl_stgy_restart_prog_inv_def by fast
-    subgoal unfolding cdcl_twl_stgy_restart_prog_inv_def by fast
-    subgoal unfolding cdcl_twl_stgy_restart_prog_inv_def by fast
-    subgoal unfolding cdcl_twl_stgy_restart_prog_inv_def
-      by (simp add: no_step_cdcl_twl_cp_no_step_cdcl\<^sub>W_cp)
-    subgoal by fast
-    subgoal for ebrk brk T m x ac bc
-      by (rule restart_prog_early_spec)
-    subgoal by (rule wf_cdcl_twl_stgy_restart_measure)
-    subgoal by fast
-    subgoal unfolding cdcl_twl_stgy_restart_prog_inv_def by fast
-    subgoal unfolding cdcl_twl_stgy_restart_prog_inv_def by fast
-    subgoal unfolding cdcl_twl_stgy_restart_prog_inv_def by fast
-    subgoal unfolding cdcl_twl_stgy_restart_prog_inv_def by fast
-    subgoal unfolding cdcl_twl_stgy_restart_prog_inv_def
-      by (simp add: no_step_cdcl_twl_cp_no_step_cdcl\<^sub>W_cp)
-    subgoal by fast
-    subgoal unfolding cdcl_twl_stgy_restart_prog_inv_def
-      by (rule restart_prog_spec[unfolded cdcl_twl_stgy_restart_prog_inv_def])
-    subgoal unfolding cdcl_twl_stgy_restart_prog_inv_def
-      by (rule final_prop[unfolded cdcl_twl_stgy_restart_prog_inv_def])
-    subgoal unfolding cdcl_twl_stgy_restart_prog_inv_def
-      by auto
+  have ref_early: \<open>cdcl_twl_stgy_restart_prog S \<le> \<Down>{((S), (ebrk, T)). S = T \<and> \<not>ebrk} (cdcl_twl_stgy_restart_prog_bounded S)\<close>
+    unfolding cdcl_twl_stgy_restart_prog_alt_def cdcl_twl_stgy_restart_prog_bounded_def
+    apply refine_rcg
+    apply assumption
+    subgoal by auto
+    subgoal by auto
+    apply (rule this_is_the_identity)
+    subgoal by auto
+    apply (rule this_is_the_identity)
+    subgoal by auto
+    apply (rule this_is_the_identity)
+    subgoal by auto
+    subgoal by auto
+    subgoal by auto
     done
+
+  show ?thesis
+    apply (rule order_trans[OF ref_early])
+    apply (rule order_trans[OF ref_two_step'])
+    apply (rule cdcl_twl_stgy_prog_bounded_spec[OF assms])
+    unfolding conc_fun_RES by fastforce
 qed
 
-*)
-definition cdcl_twl_stgy_restart_prog_bounded :: "'v twl_st \<Rightarrow> (bool \<times> 'v twl_st) nres" where
-  \<open>cdcl_twl_stgy_restart_prog_bounded S\<^sub>0 =
-  do {
-    ebrk \<leftarrow> RES UNIV;
-    (ebrk, brk, T, n) \<leftarrow> WHILE\<^sub>T\<^bsup>\<lambda>(ebrk, brk, T, m, n). cdcl_twl_stgy_restart_prog_inv S\<^sub>0 brk T m n\<^esup>
-      (\<lambda>(ebrk, brk, _). \<not>brk \<and> \<not>ebrk)
-      (\<lambda>(ebrk, brk, S, m, n).
-      do {
-        T \<leftarrow> unit_propagation_outer_loop S;
-        (brk, T) \<leftarrow> cdcl_twl_o_prog T;
-        (T, m, n) \<leftarrow> restart_prog T m n brk;
-	ebrk \<leftarrow> RES UNIV;
-        RETURN (ebrk, brk, T, m, n)
-      })
-      (ebrk, False, S\<^sub>0, size (get_all_learned_clss S\<^sub>0), 0);
-    RETURN (brk, T)
-  }\<close>
-
-lemma (in twl_restart) cdcl_twl_stgy_prog_bounded_spec:
-  assumes \<open>twl_struct_invs S\<close> and \<open>twl_stgy_invs S\<close> and \<open>clauses_to_update S = {#}\<close> and
-    \<open>get_conflict S = None\<close>
-  shows
-    \<open>cdcl_twl_stgy_restart_prog_bounded S \<le> SPEC(\<lambda>(brk, T). \<exists>m n. cdcl_twl_stgy_restart_with_leftovers (S, 0, True) m (T, n) \<and>
-        (brk \<longrightarrow> final_twl_state T))\<close>
-    (is \<open>_ \<le> SPEC ?P\<close>)
-proof -
-(*
-  have final_prop: \<open>?P (brk, T)\<close>
-    if
-     inv: \<open>case (brk, T, n) of  (brk, T, m) \<Rightarrow> cdcl_twl_stgy_restart_prog_inv S brk T m\<close>
-    for brk T n
-  proof -
-    have
-      \<open>twl_struct_invs T\<close> and
-      \<open>twl_stgy_invs T\<close> and
-      ns: \<open>brk \<longrightarrow> final_twl_state T\<close> and
-      twl_left_overs: \<open>cdcl_twl_stgy_restart_with_leftovers (S, 0) (T, n)\<close> and
-      \<open>clauses_to_update T = {#}\<close>
-      using that unfolding cdcl_twl_stgy_restart_prog_inv_def by auto
-    obtain S' where
-       st: \<open>cdcl_twl_stgy_restart\<^sup>*\<^sup>* (S, 0) (S', n)\<close> and
-       S'_T: \<open>cdcl_twl_stgy\<^sup>*\<^sup>* S' T\<close>
-      using twl_left_overs unfolding cdcl_twl_stgy_restart_with_leftovers_def by auto
-    then show ?thesis
-      using ns unfolding cdcl_twl_stgy_restart_with_leftovers_def prod.case apply -
-      apply (rule_tac x=n in exI)
-      apply (rule conjI)
-      subgoal by (rule_tac x=S' in exI) auto
-      subgoal by auto
-      done
-  qed*)
-thm cdcl_twl_stgy_restart_prog_inv_def
-thm wf_cdcl_twl_stgy_restart_measure_early
-  show ?thesis
-    supply RETURN_as_SPEC_refine[refine2 del]
-    unfolding cdcl_twl_stgy_restart_prog_bounded_def full_def
-    apply (refine_vcg
-        WHILEIT_rule[where
-           R = \<open>{((ebrk, brkT, T, n, n'), (ebrk, brkS, S, m, m')).
-                  twl_struct_invs S \<and> cdcl_twl_stgy_restart_with_leftovers1 (S, m, brkS)
-                  (T, n, brkT)} \<union>
-                {((ebrkT, brkT, T), (ebrkS, brkS, S)). S = T \<and> (ebrkT \<or> brkT) \<and> (\<not>brkS \<and> \<not>ebrkS)}\<close>];
-        remove_dummy_vars)
-    subgoal
-      by (rule wf_cdcl_twl_stgy_restart_measure_early)
-    subgoal using assms unfolding cdcl_twl_stgy_restart_prog_inv_def
-      by (auto intro: cdcl_twl_stgy_restart_with_leftovers_refl)
-    subgoal unfolding cdcl_twl_stgy_restart_prog_inv_def by fast
-    subgoal unfolding cdcl_twl_stgy_restart_prog_inv_def by fast
-    subgoal unfolding cdcl_twl_stgy_restart_prog_inv_def by fast
-    subgoal unfolding cdcl_twl_stgy_restart_prog_inv_def by fast
-    subgoal unfolding cdcl_twl_stgy_restart_prog_inv_def
-      by (simp add: no_step_cdcl_twl_cp_no_step_cdcl\<^sub>W_cp)
-    subgoal by fast
-    subgoal for ebrk brk T m x ac bc ad bd
-      by (rule restart_prog_early_spec)
-    subgoal
-      unfolding cdcl_twl_stgy_restart_prog_inv_def prod.case
-      by (rule final_prop[unfolded prod.case cdcl_twl_stgy_restart_prog_inv_def])
-    done
-qed
 end
 
 end
